# Solving Laplace's Equation with 1 Inhomogeneous Side

As discussed in [[17.1 Physical Example of Laplace's Equation]] we can use [[Laplace's Equation]] to model heat flow in a 2D surface $D \sub \R^2$

$$ u_t = \kappa \nabla ^2 u = \kappa (u_{xx} + u_{yy}) \quad \text {for $(x,y)\in D$}, $$

^eq-17-0

where $u(x,y,t)$ is the temperature. In the $t \to \infty$ we would expect the solution to reach a steady state and thus become time independent, with $u_t \to 0$, ie

$$
\nab ^2 u = 0
$$

thus restricting $u$ in this case to be purely $u(x, y)$.

> Note that $\nab^2$ is the Laplacian, equal to $\sum_i \frac{\p}{\p x_i\p x_i}$. It is sometimes written as $\lap = \nab^2$.

Equations of this variety arise when dealing with [[Potential Field|Potential Fields]] , fluid and solid dynamics, and other circumstances. They also play a key role in solving problems involving the [[Principle of Least Action]].

## Single Side Inhomogeneous Boundary Condition

The simplest boundary problem we will consider for [[Laplace's Equation]] is when one side of the surface $D$ is non-zero with the rest zero. Starting from the generic [[14.22 Dirichlet Boundary Condition|Dirichlet Condition]],

$$
u(x, y) = f(x, y) \quad \Forall (x, y) \in \p D
$$

we define $f(x, y)$ to be,

$$
f(x, y) = \begin{cases}
f'(x)	&\text{if } x \in [0, L] = 0 \land y = 0 \\
0		&\text{otherwise.} \\
\end{cases}
$$

### Other Boundary Conditions

The inhomogeneous Neumann problem is defined similarly, with the above being replaced with,

$$
\pdiff{u}{\boldn}(x,y) = g(x,y)
\quad \Forall (x,y) \in \p D,
$$

for some given function $g$ on $\p D$, where $\partial u/\partial n \equiv \boldn \cdot \nabla u$, where $\boldn$ is the outward-pointing unit normal vector to $\partial D$. For instance if the boundary of $D$ runs along the $x$ axis, the Neumann condition involves $\partial u/\partial y$, as $\boldn = (0, 1)$ or $(0,-1)$.

## Solution to [[#Single Side Inhomogeneous Boundary Condition]]

We consider Laplace’s equation in a square with side length $L$, ie $D = (0, L) \times (0, L)$, where

$$
\nab ^2 u = u_{xx} + u_{yy} = 0

\quad \Forall (x,y)\in D,
$$

> Note that these methods work equally well on rectangular domains.

considering the boundary conditions discussed earlier with zero on three sides but $f'(x)$ on the fourth:

$$
u(x, y) = \begin{cases}
f'(x)	&\text{if } x \in [0, L] = 0 \land y = 0 \\
0		& (x, y) \in \p D \\
\end{cases}
$$

Now, following [[15.X Summary of separation of variables procedure]], we first assume [[Separation of Variables]],

$$
u(x,y)= X(x) Y(y),
$$

then applying this to the PDE we get,

$$
\frac{X''(x)}{X(x)} = - \frac {Y''(y)}{Y(y)}
$$

which since they are disjoint in parameters, implies that they must both be equal to a constant, which we label $k^2 < 0$,

$$
\begin{align}
\frac{X''(x)}{X(x)} &= -k^2 \\
\frac{Y''(y)}{Y(y)} &= k^2.
\end{align}
$$

> Similar to the arguments for the Heat and Wave equation, it can be shown that this constant must be negative #todo WHY, we have symmetry don't we? Unless we are pairing the sign with the presence of the boundary condition? But that feels wrong.

This gives us two separate ODEs which we can solve to obtain,

$$
\begin{align*}
X(x) &= C\cos(kx)  + D\sin(kx), \\
Y(y) &= A\cosh(ky) + B\sinh(ky).
\end{align*}
$$

### Applying Homogeneous Boundary Conditions

First, focusing on the case $x \in \set{0, L} \land y \in [0,L]$ (the left and right edges), we know that,

$$
X(0)Y(y) = X(L)Y(y)=0 \quad \Forall y \in [0,L]
$$

^eq-17-7

which by the [[Null Product Lemma]] gives us,

$$
X(0)=X(L)=0
$$

as before these conditions imply that $C = 0$ and $\sin (kL) = 0 \implies k = \frac{n\pi}{L}, n\in \Z$.

Plugging this back into our solution we have,

$$
u(x, y) = D\sin\(\frac{n\pi}{L} x\)\Big[
	A\cosh\(\frac{n\pi}{L} y\) +
	B\sinh\(\frac{n\pi}{L} y\)
\Big]
$$

Focusing next on $y = L$ we impose $u = 0$ implying,

$$
A \cosh\(n\pi\) + B\sinh\(n\pi\)=0.
$$

It is possible solve this in terms of $A$ and $B$, however this will lead to $\tanh$ which is... a mess. A nicer technique is to notice that,

$$
\widetilde{A} \cosh(k(L-y))\qquad \widetilde{B}\sinh(k(L-y))
$$

are also valid linearly independent solutions to the PDE, which present a much neater framing where this condition implies $\widetilde A = 0$, thus giving us,

$$
u(x,y) =
\widetilde B\sin\(\frac{n\pi}{L} x\)
\sinh\(\frac{n\pi}{L}(L - y)\), \quad n \in \Z
$$

which by considering [[11.5 Properties of Even and Odd Functions#Lemma 4]] (and dropping the tildes for ease of presentation) and taking [[14.8  Principle of superposition|Superposition]] gives us,

$$
u(x,y) =
\sum_{n \in \N } B_n \sin\(\frac{n\pi}{L} x\)
\sinh\(\frac{n\pi}{L}(L - y)\)
$$

> The product of two Odd functions being Even hence making $-n \equiv n$.

## Applying Inhomogeneous Boundary Conditions

Taking the super position of these we obtain,

$$
u(x,y) =
\sum_{n \in \N } B_n \sin\(\frac{n\pi}{L} x\)
\sinh\(\frac{n\pi}{L}(L - y)\)
$$

where at $y = 0$ we require,

$$
\sum_{n \in \N } B_n \sin\(\frac{n\pi}{L} x\)
\sinh\(n\pi\)
= f'(x)
$$

^eq-17-8

Now again considering the [[12.8 Even and Odd Periodic Extensions|Odd Periodic Extension]] of $f' : [0, L] \to \R$ to $[-L, L]$, its sine series is given by,

$$
f'(x) = \sum_{n \in \N} b_n \sin\(\frac{n\pi}{L}x\)
$$

with

$$
b_n = \frac{2}{L}\int_0^l 
	f(x)\sin\(\frac{n\pi}{L} x\)
\rd x,
$$

where we assume that $f$ is sufficiently well behaved that its Fourier series [[12.5 Fourier Convergence Theorem|Fourier Series Converges]]. From these $b_n$ we can obtain $B_n$ simply by,

$$
B_n = \frac{b_n}{\sinh(n\pi)}.
$$

## Summary

$$ B_{n} = \frac {2}{L \sinh (n\pi )}\int _{0}^{L}f\left (x\right )\sin \left (\frac {n\pi x}{L}\right )\,\mathrm {d}x, $$

then

$$  u(x,y) = \sum _{n=1}^\infty B_n \sin \left ( \frac {n\pi x}{L}\right ) \sinh \left ( \frac {n\pi }{L}(L-y)\right ) $$

satisfies the Dirichlet problem for Laplace’s equation in $(0,L)\times (0,L)$ with boundary conditions

$$ u(0,y) = u(L,y) = u(x,L) = 0, \quad \text { and} \quad u(x,0) = f(x). $$

## Example

If $f(x) \equiv 1$ then,

$$ \begin{align*} B_n&= \frac {2}{L\sinh (n\pi )}\int _{0}^{L}\sin \left (\frac {n\pi x}{L}\right )\,\mathrm {d}x\\ &=\frac {2}{n\pi \sinh (n\pi )}\left [-\cos \left (\frac {n\pi x}{L}\right )\right ]_{0}^{L} \\ &= \begin{cases} \displaystyle {\frac {4}{n\pi \sinh (n\pi )}} & n\text { odd}\\ 0 & n\text { even} \end {cases} \end{align*} $$

So

$$
u(x,y)= \sum _{n\text { odd}, \,n\geq 1}\frac {4}{n\pi }\frac {1}{\sinh \left (n\pi \right )}\sin \left (\frac {n\pi x}{L}\right )\sinh \left (\frac {n\pi \left (L-y\right )}{L}\right ). $$
