---
aliases:
- Principle of superposition
- Superposition Principle
- Superposition
---

# Principle of superposition

If $u$ and $v$ are two solutions to a [[14.5 Homogeneous PDE]] (which is thus [[14.4 Linear PDE]]), then 

$$\lambda u + \mu v$$

is also a solution for any constants $\lambda$ and $\mu$.

> #todo, move this into a more general principles of mathematics bit? Or a bit in linear algebra?

## Proof

The proof follows immediately from linearity and homogeneity. Since $L(u)=0$ and $L(v)=0$, by linearity $L(\lambda u+ \mu v)=\lambda L(u) + \mu L(v)$; therefore $L(\lambda u+ \mu v)=0$.   â–¡

## Example, Linearity of the [[Heat Equation]]

We have already encountered a homogeneous linear PDE: the 1D heat equation studied in Chapter 10:

$$ u_t = \kappa \, u_{xx}. $$

^eq-14-3

Notice that indeed this can be written in the form $L(u) = f$ in [[14.8  Principle of superposition#^eq-14-3]] if we define


$$ L := \p _t - \kappa \p _{xx}, $$

^eq-14-4

and set $f \equiv 0$.