# 9.2 Radius of Convergence of Complex Power Series

Let $\sum_{k = 0}^\infty a_k (z - z_0)^k$ be a [[Power Series]] centred at $z_0 \in \C$. Suppose that $R > 0$ is its [[Radius of Convergence]].

1.  Then for any $r < R$, the power series [[Uniform Convergence|converges uniformly]] in $B_r(z_0)$.
2.  The power series $\sum_{k = 1}^\infty k a_k (z - z_0)^{k - 1}$ also has radius of convergence $R$.
3.  The function $f : B_R(z_0) \to \C$ given by $f(z) = \sum_{k = 0}^\infty a_k (z - z_0)^k$ is [[5.4 Holomorphic Function|Holomorphic]] in $B_R(z_0)$ with $f'(z) = \sum_{k = 1}^\infty k a_k (z - z_0)^{k - 1}$. ^cc1927

## Proof

### First Statement

For the proof of the first statement, fix $r < R$ and set $M_k = |a_k|r^k$. Then $\sum_{k = 0}^\infty M_k < \infty$. Since $|a_k(z - z_0)^k| \le |a_k| r^k = M_k$ for every $z \in B_r(z_0)$, the [[9.1 Weierstrass M-test|Weierstrass M-test]] implies uniform convergence in $B_r(z_0)$.

### Second Statement

For the proof of the second statement, we recall that

$$
R = \frac{1}{\limsup_{k \to \infty} |a_k|^{1/k}}.
$$

Let $R'$ be the radius of convergence of $\sum_{k = 1}^\infty k a_k (z - z_0)^{k - 1}$. For any $z \neq z_0$, convergence of $\sum_{k = 1}^\infty k a_k (z - z_0)^{k - 1}$ is equivalent to convergence of $\sum_{k = 1}^\infty k a_k (z - z_0)^k$, as every term is multiplied by $z - z_0$. Hence $R'$ coincides with the radius of convergence of the second power series. That is,

$$
R' = \frac{1}{\limsup_{k \to \infty} (k|a_k|)^{1/k}}.
$$

But as $k^{1/k} = e^{(\log k)/(k + 1)} \to 1$ as $k \to \infty$, we see that $R' = R$.

### Third Statement

Finally, in order to prove the third statement, we use [[7.5 Convergence of Holomophric Functions and their Derivatives]].

The functions 

$$ f_K(z) = \sum_{k = 0}^K a_k (z - z_0)^k $$

are polynomials, so they are [[5.4 Holomorphic Function|Holomorphic]] and 

$$ f_K'(z) = \sum_{k = 1}^K ka_k(z - z_0)^{k - 1}. $$ 

Furthermore, we know that for any $r \in (0, R)$, the functions $f_K$ converge to $f$ and $f_K'$ [[Uniform Convergence|converge uniformly]] in $B_r(z_0)$ to $\sum_{k = 1}^\infty k a_k (z - z_0)^{k - 1}$ as $K \to \infty$. 

[[7.5 Convergence of Holomophric Functions and their Derivatives]] therefore implies that 

$$
f'(z) = \sum_{k = 1}^\infty k a_k (z - z_0)^{k - 1}
$$

in $B_r(z_0)$. As this is true for any $r < R$, the formula holds in fact in $B_R(z_0)$.