# Existence of dâ€™Alembert forms for Wave Equation Solutions

The [[Separation of Variables]] technique work well for simple domains such as rectangles and circles. However on the infinite 1D line the [[Wave Equation]] admits solutions which have a different, but interesting form.

We will consider the 1D wave equation for $u(x, y): \R \times \R \to \R$, ie not restricted to a given finite range, such that,


## Theorem

Every solution of the [[#^infinite-wave-equation|wave equation]]

$$
u_{tt} = c^2 u_{xx} \qquad x \in \R.
$$

^infinite-wave-equation

can be written in [[d'Alembert Forms|d'Alembert Form]] aka as the superposition of two ***arbitrary*** **twice-differentiable** functions,

$$
u(x,t) = F(\xi) + G(\eta) = F(x - ct) + G(x + ct)
$$

^eq-19-1

with,

$$
\begin{align}
\xi &= x - ct \\
\eta &= x + ct.
\end{align}
$$
^vars

### Proof

Given a solution $u(x, t)$ we we will try to find a solution $U(\xi, \eta)$ such that,

$$
u(x, t) = U(\xi(x, t), \eta(x, t))
$$

that satisfies the [[#^infinite-wave-equation|wave equation]].

By the chain rule we have:

$$
\begin{align}
\pp{u}{x} &=
	\pp{U}{\xi}  \pp{\xi}{x} +
	\pp{U}{\eta} \pp{\eta}{x} \\
&= \pp{U}{\xi} + \pp{U}{\eta},
\end {align}
$$

and

$$
\begin{align}
\pp{u}{t} &=
	\pp{U}{\xi}  \pp{\xi}{t} +
	\pp{U}{\eta} \pp{\eta}{t} \\
&= \pp{U}{\xi}(-c) + \pp {U}{\eta}(c).
\end {align}
$$

where we have values for the differentials of $\xi$ & $\eta$ from [[#^vars|their definitions above]]. Writing this more compactly in operator notation,

$$
\begin{align}
\p_x u &=   (\p_\xi  + \p_\eta ) U, \\
\p_t u &= c (-\p_\xi + \p_\eta ) U.
\end{align}
$$

It follows that for second derivatives we have similarly

$$
\begin{align}
\p_{xx} u 
&= (\p_\xi + \p_\eta )^2 U \\
&= (\p_\xi^2 + 2\p_\xi \p_\eta + \p_\eta^2) U,\\

\\

\p_{tt} u
&= [c (-\p_\xi + \p_\eta )]^2 U \\
&= c^2 (\p_\xi^2 - 2\p_\xi \p_\eta + \p_\eta^2) U,\\
\end{align}
$$

which since we know $u$ is a solution to the wave equation we obain,

$$
c^2 (\p_\xi^2 - 2\p_\xi \p_\eta + \p_\eta^2) U
=
c^2 (\p_\xi^2 + 2\p_\xi \p_\eta + \p_\eta^2) U.
$$

from which it follows quickly that

$$
\frac{\p^2 U}{\p \eta \p \xi } = 0,
$$

which is the wave equation re-expressed in these new coordinates.

This equation can be much easier to work with however as we can integrate over the two variables simply giving us (first by $\xi$),

$$ \pp{U}{\eta} = q(\eta). $$

and finally by $\eta$

$$ U = F(\xi ) + G(\eta ), $$

which thus completes our theorem.




