# Explicit Solution from Boundary Conditions

Let $u(x,t)$ be the solutions to the wave equation posed on an infinite string and described by the system,

$$
\begin{align}
u_{tt} &= c^2 u_{xx}, \\
u(x, 0) &= f(x), \\
u_t(x, 0) &= g(x),
\end{align}
$$

 for $x\in (-\infty, \infty)$ and $t > 0$. Then the solution $u(x,t)$ is given by d’Alembert’s formula:

$$
u(x,t) = \frac12 \bigg[
	f(x - ct) + f(x + ct)
\bigg] + \frac{1}{2c} \int_{x - ct}^{x + ct} g(s) \rd s.
$$
^das-formula

In the special case where the initial velocity is identically zero, i.e. $g(x) \equiv 0$, then

$$
u(x,t) = \frac12 \bigg[ f(x - ct) + f(x + ct) \bigg],
$$

which shows that the solution is given by the shape of the initial displacement which splits into a right-traveling wave and a left-traveling wave of half the initial amplitude but the same shape.

## Proof

By Theorem 19.1 the solution is given by functions $F$ and $G$ such that

$$ u(x,t) = F(x - ct) + G(x + ct). $$

Now we apply the initial conditions. Notice first (as we have seen above already in fact) that by the chain rule the time derivative is

$$
\pp {u}{t}(x,t) = -cF’(x - ct) + cG’(x + ct).
$$

Applying the two initial conditions (19.6b) and (19.6c) at $t = 0$ we obtain the two equations

$$
\begin{align}
F(x) + G(x) &= f(x), \\
-cF'(x) + cG'(x) &= g(x).
\end{align}
$$

Integrating the second equation gives

$$
-F(x) + G(x) = \frac {1}{c} \int _0^x g(s) \, \rd {s} + a,
$$

where $a$ is constant and $s$ is just a dummy integration variable. Now we subtract this equation from, and add it to, the first equation to obtain

$$ \begin{align} F(x) & = \frac {1}{2}\left [ f(x) - \frac {1}{c}\int _0^x g(s) \, \rd {s} - a\right ], \\ G(x) & = \frac {1}{2}\left [ f(x) + \frac {1}{c}\int _0^x g(s) \, \rd {s} + a\right ]. \end{align} $$

Since the solution to the problem is given by $u(x,t)=F(x - ct) + G(x + ct)$ we have derived the solution in the form

$$ u(x,t) = \frac {1}{2}\left [f(x - ct) + f(x + ct)\right ] + \frac {1}{2c} \int _{x-ct}^{x+ct} g(s) \rd {s}. $$


