# 6.3 Uniqueness property of PGFs

We now show that the PGF determines the distribution of $X$.

Theorem 29 (Extracting probabilities from the pgf)
The pgf, $G_{X}$, of a random variable $X$ uniquely determines the
distribution of $X$ by

$$
\begin{align}
ℙ(X = k) & = & \frac{G_{X}^{(k)} (0)}{k !} & text{}
\end{align}
$$

for $k=0,1,2,…⁡$ where
$G_{X}^{(0)}(s)=G_{X}(s )$ and
$G_{X}^{(k)}(s)=\frac{d^{k}}{d s^{k}}G_{X}(s )$.

Proof: Noting that

$$
\begin{align}
G_{X}(s)=\sum_{x = 0}^{\infty}s^{x}ℙ(X = x)=ℙ(X = 0)+sℙ(X = 1)+s^{2}ℙ(X = 2)+\dots  & & & text{}
\end{align}
$$

then $G_{X}(0)=ℙ(X = 0 )$ whilst, as in
equation ([6.1](nose21.htm#x34-59004r6.1)),

$$
\begin{align}
\frac{d^{k}}{d s^{k}}G_{X}(s) & = & \sum_{x = 0}^{\infty}(\frac{d^{k}}{d s^{k}} s^{x})ℙ(X = x) & \text{} \\ & = & \sum_{x = k}^{\infty}x(x - 1)\dots (x - k + 1)s^{x - k}ℙ(X = x) & \text{} \\ & = & k!ℙ(X = k)+\sum_{x = k + 1}^{\infty}x(x - 1)\dots (x - k + 1)s^{x - k}ℙ(X = x) & text{}
\end{align}
$$

so that, evaluating at $s=0$, gives

$$
\begin{align}
G_{X}^{(k)}(0) & = & k!ℙ(X = k) & text{}
\end{align}
$$

and the result thus follows by rearrangement. $square$

Corollary 18 (Uniqueness property)
Suppose that $X$ and $Y$ have pgfs $G_{X}$ and $G_{Y}$ respectively and
$G_{X}(s)=G_{Y}(s )$ for all
$s\in[ 0, 1 right]$ then
$ℙ(X = k)=ℙ(Y = k )$ for $k=0,1,2,…⁡$ so that
$X$ and $Y$ have the same distribution.

Proof: If $G_{X}(s)=G_{Y}(s )$ for all
$s\in[ 0, 1 right]$ then
$G_{X}^{(k)}(s)=G_{Y}^{(k)}(s )$
for all $k=0,1,2,…⁡$. In particular,
$G_{X}^{(k)}(0)=G_{Y}^{(k)}(0 )$
so that, from Theorem [29](#x35-6000129),
$ℙ(X = k)=ℙ(Y = k)$. $square$

Thus, specifying the pgf is equivalent to specifying the probability
distribution and we can use the pgf to identify the distribution.

Example 64 Suppose that a random variable $Y$ has pgf
$G_{Y}(s)=frac{s}{2 - s}$ find the distribution of $Y$ .

Note that

$$
\begin{align}
\frac{s}{2 - s} & = & \frac{s \frac{1}{2}}{1 - s \frac{1}{2}} & text{}
\end{align}
$$

and, from Example [62](nose20.htm#x33-5800562), if
$XsimGeom(p )$ then
$G_{X}(s)=\frac{s p}{1 - s (1 - p )}$. Thus, by
the uniqueness property, $YsimGeom(1 / 2 )$.

Example 65 Suppose that $X$ has pgf
$G_{X}(s)=\frac{((1 + s))^{2}}{4}$
. Find the distribution of $X$.

Note that

$$
\begin{align}
\frac{d}{d s}G_{X}(s)=\frac{1 + s}{2},\frac{d^{2}}{d s^{2}}G_{X}(s)=\frac{1}{2},\frac{d^{k}}{d s^{k}}G_{X}(s)=0 & & & text{}
\end{align}
$$

for $k=3,4,…⁡$. Thus,

$$
\begin{align}
ℙ(X = 0)=G_{X}(0)=\frac{1}{4},ℙ(X = 1)=\frac{G_{X}^{(1)} (0)}{1 !}=\frac{1}{2},ℙ(X = 2)=\frac{G_{X}^{(2)} (0)}{2 !}=\frac{1}{4} & & & text{}
\end{align}
$$

with $ℙ(X = k )=0$ for $k=3,4,…⁡$. Note that these
probabilities are exactly those for $XsimB(2, 1 / 2 )$.

\


