# 6.4 Finding the distribution of sums of independent random variables

Much of probability and statistics is concerned with sums of independent
random variables. Probability generating functions provide a powerful
tool for finding the probability distribution of such sums.

Theorem 30 (Pgf of a sum of independent random variables)
If $X$ and $Y$ are independent random variables with pgfs $G_{X}$ and
$G_{Y}$ respectively then the pgf, $G_{X + Y}$, of $X+Y$ is

$$
\begin{align}
G_{X + Y}(s)=G_{X}(s)G_{Y}(s). & & & text{}
\end{align}
$$

Proof: From Corollary [12](nose17.htm#x29-5100112), if $X$ and $Y$ are
independent then
$ùîº(s^{X + Y})=ùîº(s^{X})ùîº(s^{Y} )$
so that

$$
\begin{align}
G_{X + Y}(s)=ùîº(s^{X + Y})=ùîº(s^{X})ùîº(s^{Y})=G_{X}(s)G_{Y}(s). & & & text{}
\end{align}
$$

$square$

Notice that this result can be extended to $n$ independent random
variables $X_{1},‚Ä¶‚Å°,X_{n}$, with individual pgfs
$G_{X_{i}}(s )$, so that if
$Y=(\sum ‚Å°)_{i = 1}^{n}X_{i}$ then

$$
\begin{align}
G_{Y}(s) & = & \prod_{i = 1}^{n}G_{X_{i}}(s). & \text{(6.2)}\text{}text{}
\end{align}
$$

Example 66 Suppose that $XsimPo(\lambda )$ and
$YsimPo(\mu )$ are independent. Find the distribution of
$X+Y$ .

If $XsimPo(\lambda )$ then

$$
\begin{align}
G_{X}(s) & = & \sum_{x = 0}^{\infty}s^{x}\frac{(\lambda)^{x}}{x !}e^{- \lambda} & \text{} \\ & = & e^{- \lambda}e^{s \lambda}\sum_{x = 0}^{\infty}\frac{((s \lambda))^{x}}{x !}e^{- s \lambda}=e^{\lambda (s - 1)} & text{}
\end{align}
$$

as the sum is the sum of $Po(s \lambda )$ probabilities. By
the uniqueness of pgfs,
$G_{Y}(s)=e^{\mu (s - 1 )}$ so that

$$
\begin{align}
G_{X + Y}(s) & = & G_{X}(s)G_{Y}(s) & \text{} \\ & = & e^{\lambda (s - 1)}e^{\mu (s - 1)}=e^{(\lambda + \mu) (s - 1)}. & text{}
\end{align}
$$

Thus, by the uniqueness of pgfs, $X+YsimPo(\lambda + \mu )$.

Example 67 Suppose that $XsimB(n, p )$. Use the uniqueness
property of pgfs to find the pgf of $X$.

Note that $X$ is the sum of $n$ independent Bernoulli trials, each with
probability of success $p$. That is
$X=(\sum ‚Å°)_{i = 1}^{n}X_{i}$ where each
$X_{i}simBern(p )$ and $X_{1},‚Ä¶‚Å°,X_{n}$ are independent.
From Example [61](nose20.htm#x33-5800361) we have that

$$
\begin{align}
G_{X_{i}}(s) & = & (1 - p)+sp. & text{}
\end{align}
$$

Using equation ([6.2](#x36-61004r6.2)),

$$
\begin{align}
G_{X}(s) & = & \prod_{i = 1}^{n}G_{X_{i}}(s) & \text{} \\ & = & \prod_{i = 1}^{n}\{ (1 - p) + s p \}=(\{ (1 - p) + s p \})^{n}. & text{}
\end{align}
$$

We know, by construction, that $XsimB(n, p )$ and so, by
the uniqueness of pgfs, the pgf of $XsimB(n, p )$ is
$G_{X}(s)=(\{ (1 - p) + s p \})^{n}$.

Notice that for $n=2$ and $p=1/2$ we find
$G_{X}(s)=\frac{((1 + s))^{2}}{4}$
which matches with our observation in Example
[65](nose22.htm#x35-6000965).

\
\
