### [[6.3 Properties of the Divergence]]

If $\boldF$ and $\boldG$ are differentiable vector fields, $\phi (\boldx )$ is a differentiable scalar field, and $\lambda$ and $\mu$ are constants, then



$$  \nabla \cdot (\lambda \boldF + \mu \boldG ) = \lambda \nabla \cdot \boldF + \mu \nabla \cdot \boldG , $$

and

$$  \nabla \cdot (\phi \boldF ) =(\nabla \phi )\cdot \boldF + \phi (\nabla \cdot \boldF ). $$

#### Proof

For (6.3), use the definition of the divergence (6.1) and the linearity of differentiation. For (6.4), use the definition of the divergence (6.1) and the product rule. Observe that these proofs are even shorter using index notation!