# 11.2

Suppose that $\gamma : [a, b] \to \C$ is a [[6.1 Contours|Closed Contour]] and $\Gamma = \gamma([a, b])$ is the [[6.10 Curve of the Contour]]. If $z \in \C \setminus \Gamma$, then,

- $W(\gamma, z)$ is an integer.
- Furthermore, the function $W(\gamma, \cdot) : \C \setminus \Gamma \to \mathbb{Z}$ is continuous.

## Proof

Since $\gamma$ is a contour, it is piecewise continuously differentiable. That is, it is continuous and there exist $t_0, \dotsc, t_K$ with $a = t_0 < \dotsb < t_K = b$ such that $\gamma$ is continuously differentiable in $(t_{k - 1}, t_k)$ and $\gamma'$ has a continuous extension to $[t_{k - 1}, t_k]$ for $k = 1, \dotsc, K$.

For $t \in [a, b]$, define

$$
\begin{equation*} F(t) = \int_a^t \frac{\gamma'(s)}{\gamma(s) - z} \, ds. \end{equation*}
$$

Then $F(b) = 2\pi i W(\gamma, z)$. The function $F$ is continuous, and in each of the intervals $(t_{k - 1}, t_k)$, it is differentiable with

$$
\begin{equation*} F'(t) = \frac{\gamma'(t)}{\gamma(t) - z} \end{equation*}
$$

by the fundamental theorem of calculus. Now define $G(t) = e^{-F(t)} (\gamma(t) - z)$. Then we compute

$$
\begin{equation*} G'(t) = e^{-F(t)} \gamma'(t) -F'(t) e^{-F(t)} (\gamma(t) - z) = 0 \end{equation*}
$$

in $(t_{k - 1}, t_k)$. Hence $G$ is constant in these intervals. It is also continuous in $[a, b]$, and therefore it is constant in $[a, b]$. In other words, there exists a constant $c \in \mathbb{R}$ such that

$$
\begin{equation*} e^{-F(t)} (\gamma(t) - z) = c \end{equation*}
$$

for all $t \in [a, b]$. So $\gamma(t) - z = ce^{F(t)}$. Clearly $c \neq 0$, since $z \not\in \Gamma$.

Since $\gamma$ is a closed contour, it satisfies $\gamma(a) = \gamma(b)$. By the above formula, this means that

$$
\begin{equation*} c = ce^{F(a)} = ce^{F(b)}. \end{equation*}
$$

As $c \neq 0$, we conclude that $e^{F(b)} = 1$. Therefore, there exists $\ell \in \mathbb{Z}$ such that $F(b) = 2\pi \ell i$. Hence $W(\gamma, z) = \frac{F(b)}{2\pi i} = \ell \in \mathbb{Z}$.

Next we prove continuity of $W(\gamma, \cdot)$ on $\C \setminus \Gamma$. Consider $z_0, z \in \C \setminus \Gamma$. Then

$$
\begin{equation*} \begin{split} W(\gamma, z) - W(\gamma, z_0) & = \frac{1}{2\pi i} \int_\gamma \left(\frac{1}{w - z} - \frac{1}{w - z_0}\right) \, dw \\ & = \frac{1}{2\pi i} \int_\gamma \frac{z - z_0}{(w - z)(w - z_0)} \, dw. \end{split} \end{equation*}
$$

Let $r = \mathop{\mathrm{dist}}(z_0, \Gamma)$. If $|z - z_0| \le \frac{r}{2}$, then $\mathop{\mathrm{dist}}(z, \Gamma) \ge \frac{r}{2}$ and it follows that

$$
\begin{equation*} \max_{w \in \Gamma} \left|\frac{z - z_0}{(w - z)(w - z_0)}\right| \le \frac{2}{r^2} |z - z_0|. \end{equation*}
$$

According to Lemma [6.2](estimates-and-convergence.html#lem:ML), this implies that

$$
\begin{equation*} |W(\gamma, z) - W(\gamma, z_0)| \le\frac{L(\gamma)}{\pi r^2} |z - z_0|. \end{equation*}
$$

In particular, if we let $z \to z_0$, then $W(\gamma, z) \to W(\gamma, z_0)$.