MA10207 – Analysis 1 (Semester 2)
=================================

#### 3.5 Properties of the integral

In this section we discuss the additivity and linearity of the integral, as well as some related properties.

We collect all results ﬁrst and give some proofs later on.

Theorem 3.23. 

Let $a< b$ and $f \colon [a,b]\to \R$ be a bounded function. For any $a<c<b$, $f$ is integrable in $[a,b]$ if and only $f$ is integrable in $[a,c]$ and $f$ is integrable in $[c,b]$. In this case we have


$$
 \int _a^b f = \int _a^c f + \int _c^b f. 
$$

The previous theorem motivates the following notation.

Deﬁnition 3.24. 

Let $A, B \in \R$ with $A < B$ and $f\colon [A,B]\to \R$ be integrable. For any $a,b\in [A,B]$, $a\leq b$ we deﬁne


$$
 \int _a^a f = 0 , \quad \int _b^a f = - \int _a^b f. 
$$

With this deﬁnition we then have that for any $a,b,c\in [A,B]$



$$
 \being{align} \label {general additivity} \int _a^b f = \int _a^c f + \int _c^b f . \end{align} 
$$
^eq-3-13


Theorem 3.25 (Linearity of the integral). 

Let $f,g\colon [a,b]\to \R$ be integrable and $\alpha \in \R$.

(a) Then $f+g$ is integrable and



$$
 \being{align} \label {integral-sum} \int _a^b (f+g) = \int _a^b f + \int _a^b g . \end{align} 
$$
^eq-3-14


(b) $\alpha f$ is integrable and


$$
 \int _a^b (\alpha f) = \alpha \int _a^b f 
$$

Theorem 3.26. 

Let $f,g\colon [a,b]\to \R$ be integrable functions. Then $f\cdot g$ is integrable in $[a,b]$.

Theorem 3.27. 

Let $f,g\colon [a,b]\to \R$ be integrable, such that $f(x)\leq g(x)$ for all $x\in [a,b]$. Then


$$
 \int _a^b f \leq \int _a^b g. 
$$

Theorem 3.28. 

Let $f\colon [a,b]\to \R$ be integrable. Then $|f|$ is integrable in $[a,b]$ and



$$
 \being{align} \label {ineq int abs value} \Bigl |\int _a^b f \Bigr |\leq \int _a^b |f| . \end{align} 
$$
^eq-3-15


Proof of Theorem 3.23. First suppose that $f$ is integrable in $[a,b]$ and let $c\in (a,b)$.

We will use the Cauchy criterion to verify that $f$ is integrable in $[a,c]$ and in $[c,b]$.

Let $\varepsilon >0$. Since $f$ is integrable in $[a,b]$, there exists a subdivision $Q$ of $[a,b]$ such that


$$
 U(f,Q) - L(f,Q) < \varepsilon . 
$$

Let $\tilde Q = Q \cup \{c\}$, which is a reﬁnement of $Q$. Therefore, by Lemma 3.6,


$$
 U(f,\tilde Q) - L(f,\tilde Q) \leq U(f,Q) - L(f,Q) < \varepsilon . 
$$

Let us write


$$
 \tilde Q = \{ x_0, x_1,\ldots ,x_n\}, \quad x_0 = a < x_1 < \ldots < x_n = b 
$$

Since $c \in \tilde Q$, we must have $c = x_k$ for some $k\in \{1,2,\ldots ,n-1\}$. We deﬁne


$$
 P_1 = \{ x_0, x_1,\ldots ,x_k\}, \quad P_2 = \{ x_k, x_1,\ldots ,x_n\}, 
$$

and note that $P_1$ is a subdivision of $[a,c]$ and that $P_2$ is a subdivision of $[c,b]$.

We have


$$
 \begin {aligned} & U(f,P_1) - L (f,P_1) +U(f,P_2) - L (f,P_2) \\ &\quad = \sum _{i=1}^n \Bigl ( \sup _{[x_{i-1},x_i]} f - \inf _{[x_{i-1},x_i]} f \Bigr ) (x_i-x_{i-1}) \\ &\quad = U(f,\tilde Q) - L (f,\tilde Q ) <\varepsilon . \end {aligned} 
$$

Since $U(f,P_1) - L (f,P_1)\geq 0$ and $U(f,P_2) - L (f,P_2)\geq 0$ by Lemma 3.4, we conclude that



$$
 \being{align*} U(f,P_1) - L (f,P_1)< \varepsilon , \quad U(f,P_2) - L (f,P_2)<\varepsilon . \end{align*} 
$$
^eq-3-16
 This shows that $f$ is integrable on $[a,c]$ and on $[c,b]$.

Moreover, using [[#^eq-3-6]]



$$
 \being{align*} \int _a^c f + \int _c^b f -2 \varepsilon \leq L(f,P_1) + L(f,P_2) = L(f,\tilde Q) \leq \int _a^b f \end{align*} 
$$
^eq-3-16
 and [[#^eq-3-6]] again



$$
 \being{align*} \int _a^b f\leq L(f,\tilde Q) + \varepsilon = L(f,P_1) + L(f,P_2) + \varepsilon \leq \int _a^c f + \int _c^b f + 2 \varepsilon . \end{align*} 
$$
^eq-3-16
 Combining these inequalities we ﬁnd that



$$
 \being{align*} \int _a^c f + \int _c^b f -2 \varepsilon \leq \int _a^b f \leq \int _a^c f + \int _c^b f + 2 \varepsilon . \end{align*} 
$$
^eq-3-16
 Since $\varepsilon >0$ is arbitrary, we deduce that


$$
 \int _a^b f = \int _a^c f + \int _c^b . 
$$

Now assume that $f$ is integrable on $[a.c]$ and on $[c,b]$. Let $\varepsilon >0$. Let $P_1$ be a subdivision of $[a,c]$ such that


$$
 U(f,P_1) - L(f,P_1) < \frac {\varepsilon }{2} 
$$

and let $P_2$ be a subdivision of $[c,b]$ such that


$$
 U(f,P_2) - L(f,P_2) < \frac {\varepsilon }{2} . 
$$

Then $P = P_1 \cup P_2$ is a subdivision of $[a,b]$ and


$$
 U(f,P)-L(f,P) = U(f,P_1)-L(f,P_1) + U(f,P_2)-L(f,P_2) < \varepsilon . 
$$

This proves that $f$ is integrable in $[a,b]$.

 □

Proof of Theorem 3.25.

We prove (a) and leave (b) as an exercise.

We will use the Cauchy criterion, but ﬁrst we prove that for any subdivision $P$ of $[a,b]$ we have



$$
 \being{align} \label {ineq-upper-sum} U(f+g,P) & \leq U(f,P) + U(g,P) \\ \label {ineq-lower-sum} L(f+g,P) & \geq L(f,P) + L(g,P) . \end{align} 
$$
^eq-3-16


Indeed, let us write


$$
 P = \{x_0,x_1,\ldots ,x_n\}, \quad a = x_0 < x_1 < \ldots < x_n = b , \quad I_i = [x_{i-1},x_i]. 
$$

We observe that



$$
 \being{align} \label {ineq-sup} \sup _{I_i}(f+g) \leq \sup _{I_i}f + \sup _{I_i} g . \end{align} 
$$
^eq-3-18
 Indeed, for $x\in I_i$:


$$
 f(x) + g(x) \leq \sup _{I_i} f + \sup _{I_i} g . 
$$

Taking the supremum over $x\in I_i$ we ﬁnd that [[#^eq-3-19]] holds.

Using [[#^eq-3-19]] we obtain


$$
 \begin {aligned} U(f+g,P) &= \sum _{i=1}^n \sup _{I_i}(f+g) |I_i| \leq \sum _{i=1}^n ( \sup _{I_i} f + \sup _{I_i} g )|I_i| \\ & = U(f,P)+ U(g,P) , \end {aligned} 
$$

and this proves [[#^eq-3-17]]. In a similar way we can prove that [[#^eq-3-18]].

Let $\varepsilon >0$ be given and $P_1$, $P_2$ be subdivisions of $[a,b]$ such that


$$
 U(f,P_1) - L(f,P_1) < \frac {\varepsilon }{2} , \quad U(g,P_2) - L(g,P_2) < \frac {\varepsilon }{2}. 
$$

Let $P = P_1 \cup P_2$, which is a reﬁnement of $P_1$ and $P_2$. Then



$$
 \being{align} \label {ineq-int-sum1} U(f,P) - L(f,P) < \frac {\varepsilon }{2} , \quad U(g,P) - L(g,P) < \frac {\varepsilon }{2}. \end{align} 
$$
^eq-3-19
 Using the above inequality and [[#^eq-3-17]], [[#^eq-3-18]] we ﬁnd that



$$
 \being{align} \label {ineq-int-sum2} U(f+g,P)-L(f+g,P) \leq U(f,P) - L(f,P) + U(g,P)- L(g,P) < \varepsilon . \end{align} 
$$
^eq-3-20
 This proves that $f+g$ satisﬁes the Cauchy criterion and hence it is Riemann integrable.

Next we prove [[#^eq-3-15]]. For this, let $\varepsilon >0$ and $P$ a subdivision of $[a,b]$ such that [[#^eq-3-20]] and [[#^eq-3-21]] hold. Using Remark 3.14 we obtain



$$
 \being{align*} \int _a^b (f+g) \leq U(f+g,P) \leq U(f,P)+ U(g,P) \leq \int _a^b f +\int _a^b g + \varepsilon . \end{align*} 
$$
^eq-3-21
 Similarly



$$
 \being{align*} \int _a^b (f+g) \geq L(f+g,P) \geq L(f,P)+ L(g,P) \geq \int _a^b f +\int _a^b g - \varepsilon . \end{align*} 
$$
^eq-3-21
 Combining the previous inequalities we ﬁnd that


$$
 \int _a^b f +\int _a^b g - \varepsilon \leq \int _a^b (f+g) \leq \int _a^b f +\int _a^b g + \varepsilon . 
$$

Since $\varepsilon >0$ is arbitrary we conclude that


$$
 \int _a^b (f+g) = \int _a^b f +\int _a^b g . 
$$

 □

Proof of Theorem 3.28.

Let $\varepsilon >0$ and $P = \{x_0,x_1,\ldots ,x_n\}$ be a subdivision of $[a,b]$ such that


$$
 U(f,P) - L(f,P) < \varepsilon . 
$$

We assume $x_0= a <x_1<\ldots < x_n$ and let $I_j = [x_{j-1},x_j]$.

Then



$$
 \being{align*} U(|f|,P) - L(|f|,P) &= \sum _{j=1}^n ( \sup _{I_j} |f| - \inf _{I_j} |f| ) |I_j|. \end{align*} 
$$
^eq-3-21


We claim that



$$
 \being{align} \label {ineq4} \sup _{I_j} |f| - \inf _{I_j} |f| \leq \sup _{I_j} f - \inf _{I_j} f. \end{align} 
$$
^eq-3-21
 To prove this, we ﬁrst observe that


$$
 |\, |a|-|b| \, | \leq |a-b|. 
$$

Let $x,y \in I_j$ and assume that $f(x) \geq f(y)$. Then



$$
 \being{align} \label {ineq3} |f(x)|- |f(y)|\leq |f(x)-f(y)| = f(x) - f(y) \leq \sup _{I_j} f - \inf _{I_j} f. \end{align} 
$$
^eq-3-22
 In a similar way we obtain the same inequality if $f(y) \geq f(x)$. Taking supremum in $x$ and $y$ in $I_j$ in [[#^eq-3-23]] we obtain [[#^eq-3-22]].

Using [[#^eq-3-22]] we ﬁnd that



$$
 \being{align*} U(|f|,P) - L(|f|,P) &\leq \sum _{j=1}^n ( \sup _{I_j} f - \inf _{I_j} f ) |I_j| < \varepsilon . \end{align*} 
$$
^eq-3-23
 This shows that $|f|$ is integrable in $[a,b]$.

Let us prove the inequality [[#^eq-3-16]] We have $f(x) \leq |f(x)|$ for all $x\in [a,b]$. Using Theorem 3.27 we deduce that


$$
 \int _a^b f \leq \int _a^b | f |. 
$$

In a similar way we obtain


$$
 -\int _a^b f \leq \int _a^b | f | , 
$$

and the two previous inequalities imply [[#^eq-3-16]].  □