MA10207 – Analysis 1 (Semester 2)
=================================

#### 2.2 Derivatives of basic functions

Theorem 2.7. 

Let $n \in \N$ and $p\colon \R \to \R$ be given by

$$ p(x) = \sum _{k=0}^n a_k x^k , $$

where $a_0,\ldots ,a_n\in \R$. Then for any $c\in \R$, $p$ is diﬀerentiable at $c$, and

$$ p^\prime (c) = \sum ^{n}_{k=1} k a_k c^{k-1}. $$

Proof. We ﬁrst prove that monomials are diﬀerentiable. A monomial $m:\R \to \R$ is a function of the form

$$ m(x) = x^n $$

where $n\in \N$. Let $c\in \R$. Then


$$ \being{align*} \lim _{h\to 0}\frac {m(c+h)-m(c)}{h} &= \lim _{h\to 0}\frac {(c+h)^n-c^n}{h} \\ & =\lim _{h\to 0} \sum _{k=1}^n \binom {n}{k} c^{n-k} h^{k-1} \\ &= n c^{-1} . \end{align*} $$
^eq-2-1
 This shows that $m$ is diﬀerentiable at $c$ and $m’(c) = n c^{n-1}$.

Then the diﬀerentiability of a polynomial follows from the algebra for derivatives, Theorem 2.5.  □

Theorem 2.8. 

The functions $\exp$, $\sin$, $\cos$ deﬁned in [[#^eq-1-8]] are diﬀerentiable in $\R$ and


$$ \being{align*} \exp ’(x) = \exp (x) , \quad \sin ’(x)=\cos (x), \quad \cos ’(x) = -\sin (x). \end{align*} $$
^eq-2-1


Proof. First we prove that $\exp$ is diﬀerentiable at $c=0$. For this we derive ﬁrst the following inequality:


$$ \being{align} \label {ineq-exp2} \Bigl | \frac {\exp (x)-1}{x} -1 \Bigr | \leq e |x| , \quad \forall x\in [-1,1] , \end{align} $$
^eq-2-1
 where $e = \exp (1)$. Indeed, we start by observing that


$$ \being{align*} \exp (x) -1 &= \sum _{k=1}^\infty \frac {x^k}{k!} = x \sum _{k=0}^\infty \frac {x^k}{(k+1)!} \end{align*} $$
^eq-2-2
 and


$$ \being{align*} \frac {\exp (x)-1}{x} -1 &= \sum _{k=1}^\infty \frac {x^k}{(k+1)!} = x \sum _{k=0}^\infty \frac {x^k}{(k+2)!} \end{align*} $$
^eq-2-2


For $x\in [-1,1]$,


$$ \being{align*} \left | \sum _{k=0}^\infty \frac {x^k}{(k+2)!} \right | & \leq \sum _{k=0}^\infty \frac {1}{k ! } = e . \end{align*} $$
^eq-2-2
 and this proves [[#^eq-2-2]]. From [[#^eq-2-2]] we deduce that


$$ \being{align*} \lim _{h\to 0} \Bigl [ \frac {\exp (h)-1}{h} -1 \Bigr ]=0 \end{align*} $$
^eq-2-2
 which is the same as

$$ \lim _{h\to 0} \frac {\exp (h)-1}{h} = 1. $$

Therefore $\exp$ is diﬀerentiable at $0$ and $\exp ’(0)=1$.

Let us prove that $\exp$ is diﬀerentiable at $c\in \R$. For this recall that $\exp (x+y) = \exp (x) \exp (y)$ for all $x,y\in \R$ and therefore


$$ \being{align*} \lim _{h\to 0}\frac {\exp (c+h)-\exp (c)}{h} &= \lim _{h\to 0}\frac {\exp (c)\exp (h)-\exp (c)}{h} \\ & = \exp (c) \lim _{h\to 0}\frac {\exp (h)-\exp (0)}{h} =\exp (c). \end{align*} $$
^eq-2-2
 This shows that $\exp$ is diﬀerentiable at $c\in \R$ and $\exp ’(c) = \exp (c)$.

The proof for $\sin$ and $\cos$ are similar. We only prove the relevant inequality


$$ \being{align*} \Bigl | \frac {\sin (x)}{x}-1\Bigr | \leq e x^2 , \quad |x|\leq 1. \end{align*} $$
^eq-2-2
 Indeed, for $|x|\leq 1$, we have


$$ \being{align*} \Bigl | \frac {\sin (x)}{x}-1\Bigr | &= \Bigl | \sum _{n=0}^\infty (-1)^n \frac {x^{2n}}{(2n+1)!}-1 \Bigr | \\ &= \Bigl | \sum _{n=1}^\infty (-1)^n \frac {x^{2n}}{(2n+1)!} \Bigr | \\ & \leq x^2 \sum _{n=1}^\infty \frac {1}{(2n+1)!} \\ & \leq x^2 \sum _{n=0}^\infty \frac {1}{n!} \\ & \leq e x^2. \end{align*} $$
^eq-2-2


 □