# Laurent's Theorem

Let $U \sub \C$ be an [[Open Set]] and $f : U \to \C$ a [[5.4 Holomorphic Function|Holomorphic Function]].

For $z_0 \in \C$ and $r, R > 0$ with $r < R$, suppose that $\overline{B_R(z_0)} \setminus B_r(z_0) \sub U$.

Let $r_0 \in (r, R)$ and consider the [[6.1 Contours|Contour]],

$$
\begin{gather}
\gamma : [0, 2\pi] \\
\gamma(t) = z_0 + r_0 e^{it}
\end{gather}
$$

which can clearly be seen to be a circle radius $r_0$ around $z_0$.

Define, for $k \in \Z$,

$$
a_k = \frac{1}{2\pi i}
\int_\gamma \frac{f(w)}{(w - z_0)^{k + 1}} \rd w.
$$

Then the [[10.1 Laurent Series]] for $f$ is given as,

$$
\begin{equation} f(z) = \sum_{k = -\infty}^\infty a_k (z - z_0)^k \tag{10.1} \end{equation}
$$

for all $z \in B_R(z_0) \setminus \overline{B_r(z_0)}$.

> **Compare Contrast**: [[9.4 Power Series Expansion of Holomorphic Functions]]
> 
> Thus this can be seen as an... extension(?) of said Theorem?

## Uniqueness

This Laurent series expansion is unique in the following sense: if

$$f(z) = \sum_{k = -\infty}^\infty b_k (z - z_0)^k$$

for all $z \in B_R(z_0) \setminus \overline{B_r(z_0)}$, then $b_k = a_k$ for all $k \in \mathbb{Z}$.

## Proof

![[Laurent2.png]]

Let $A = B_R(z_0) \setminus \overline{B_r(z_0)}$. Then for any $z \in A$, we may choose $s > 0$ such that $B_s(z) \sub A$. By Theorem [[8.4 The Local Cauchy Formula]],

$$
f(z) = \frac{1}{2\pi i} \int_{\partial B_s(z)} \frac{f(w)}{w - z} \rd w
$$

where the orientation of $\partial B_s(z)$ is anticlockwise.

Now fix $\phi \in [0, 2\pi), 0 \le  r \lt \rho \le s$ such that

$$ z - z_0 = \rho e^{i\phi}. $$

Define $\tilde{r} = \rho - s$ and $\tilde{R} = \rho + s$. Consider the following contours $\gamma_1, \gamma_2, \gamma_3, \gamma_4$ (depicted in the above figure),

$$
\begin{align}

\gamma_1(t) &= z + se^{i(t + \phi - \pi)} \\
\gamma_2(t) &= z + se^{i(t + \phi)} \\

\\

\gamma_3(t) &= z_0 + \tilde{R} e^{i(t + \phi)} \\
\gamma_4(t) &= z_0 + \tilde{r} e^{i(\phi - t)} \\
\end{align}
$$

Then $\partial B_s(z)$ is parametrised by $\gamma_1 + \gamma_2$. We also consider

$$
\gamma_0 = \gamma_1 + \gamma_3 - \gamma_1 + \gamma_4.
$$

![[Laurent4.png|Homotopy between $\gamma_0$ and $\partial B_s(z)$]]
> Homotopy between $\gamma_0$ and $\partial B_s(z)$

Then, as demonstrated in the above Figure, the contour $\gamma_0$ is [[8.1 Homotopy|Homotopic]] to $\gamma_1 + \gamma_2$ in $A \setminus \{z\}$ after a suitable reparametrisation. By [[8.4 The Local Cauchy Formula]], this means that

$$
\begin{align}
f(z)

&= \frac{1}{2\pi i} \int_{\gamma_1 + \gamma_2} 
	\frac{f(w)}{w - z}
\rd w \\ 

&= \frac{1}{2\pi i} \int_{\gamma_0}
	\frac{f(w)}{w - z}
\rd w \\

&= \frac{1}{2\pi i} \int_{\gamma_3}
	\frac{f(w)}{w - z}
\rd w + \frac{1}{2\pi i} \int_{\gamma_4}
	\frac{f(w)}{w - z}
\rd w.
\end{align}
$$

### Term 1: $\gamma_3$

The term

$$
\frac{1}{2\pi i} \int_{\gamma_3} \frac{f(w)}{w - z} \rd w
$$

can now be expressed as a power series with the same arguments as in the proof of [[9.4 Power Series Expansion of Holomorphic Functions]]. We recall that

$$
\frac{f(w)}{w - z} = \sum_{k = 0}^\infty \frac{f(w)}{(w - z_0)^{k + 1}} (z - z_0)^k
$$

when $|z - z_0| < |w - z_0|$, and the convergence is uniform on $\partial B_{\tilde{R}}(z_0)$. Therefore,

$$
\frac{1}{2\pi i} \int_{\gamma_3} 
	\frac{f(w)}{w - z}
\rd w = \frac{1}{2\pi i} \sum_{k = 0}^\infty \int_{\gamma_3} \frac{f(w)}{(w - z_0)^{k + 1}} \, dw \, (z - z_0)^k.
$$

Moreover, the contour $\gamma_3$ is homotopic to $\gamma$ in $A$. Hence, using Theorem [[8.3 Cauchy Integral Theorem]] and [[9.4 Power Series Expansion of Holomorphic Functions]], we see that

$$
\frac{1}{2\pi i} \int_{\gamma_3} \frac{f(w)}{(w - z)^{k + 1}} \, dw = a_k
$$

for $k \ge 0$.

We use similar arguments for

$$
\begin{equation*} \frac{1}{2\pi i} \int_{\gamma_4} \frac{f(w)}{w - z} \, dw. \end{equation*}
$$

### Term 2: $\gamma_4$

We observe that

$$
\begin{equation*} \frac{1}{w - z} = -\frac{1}{z - z_0} \frac{1}{1 - \frac{w - z_0}{z - z_0}} = - \frac{1}{z - z_0} \sum_{\ell = 0}^\infty \left(\frac{w - z_0}{z - z_0}\right)^\ell = -\sum_{\ell = 0}^\infty \frac{(w - z_0)^\ell}{(z - z_0)^{\ell + 1}}, \end{equation*}
$$

as long as $|w - z_0| < |z - z_0|$. The substitution $k = - (\ell + 1)$ now gives

$$
\begin{equation*} \frac{1}{w - z} = - \sum_{k = -\infty}^{-1} \frac{(z - z_0)^k}{(w - z_0)^{k + 1}}. \end{equation*}
$$

The convergence is uniform on $\partial B_{\tilde{r}}(z_0)$ by the same arguments as in the proof of Theorem [9.1](analyticity-of-holomorphic-functions.html#thm:power-series-expansion). Hence

$$
\begin{equation*} \frac{1}{2\pi i} \int_{\gamma_4} \frac{f(w)}{w - z} \, dw = - \frac{1}{2\pi i} \sum_{k = -\infty}^{-1} \int_{\gamma_4} \frac{f(w)}{(w - z_0)^{k + 1}} \, dw \, (z - z_0)^k. \end{equation*}
$$

The contour $-\gamma_4$ is [[8.1 Homotopy|Homotopic]] to $\gamma$ in $A$. Hence

$$
\begin{equation*} -\frac{1}{2\pi i} \int_{\gamma_4} \frac{f(w)}{(w - z_0)^{k + 1}} \, dw = \frac{1}{2\pi i} \int_{-\gamma_4} \frac{f(w)}{(w - z_0)^{k + 1}} \, dw = a_k \end{equation*}
$$

for $k < 0$. 

### Conclusion

Combining all of these identities, we find the Laurent series expansion as above.

## Proof of Uniqueness

It remains to show that this Laurent series expansion is unique. Suppose therefore that

$$
f(z) = \sum_{k = -\infty}^\infty b_k(z - z_0)^k
$$

for all $z \in A$. Substituting this into the formulas in the statement of the theorem, we conclude that

$$
a_k = \frac{1}{2\pi i} \sum_{\ell = -\infty}^\infty b_\ell \int_{\gamma} (w - z_0)^{\ell - k - 1} \rd w
$$

for all $k \in \Z$. By the calculations from [[7.8 Local Cauchy Theorem#Example 2]], we know that

$$
\int_{\gamma} (w - z_0)^{\ell - k - 1} \rd w = 0
$$

for $k \neq \ell$; and for $k = \ell$, the integral is $2\pi i$. Therefore, we conclude that $a_k = b_k$.
