## 11.7 Orthogonality Lemma

#todo cleanup
#todo extend to $0$ case.

Let $n,m \in \Z \setminus 0$. Then the following results hold:

$$
\begin{align}
\int_{-\pi }^{\pi }\sin (nx)\cos (mx)\, \mathrm {d}x &= 0,  \\
\int _{-\pi }^{\pi }\cos (nx)\ \cos (mx)\, \mathrm {d}x &= \pi \delta _{mn},  \\
\int _{-\pi }^{\pi }\sin (nx)\ \sin (mx)\, \mathrm {d}x &= \pi \delta _{mn},  \end{align} $$
^eq-11-100

where $\delta$ is the [[Kronecker Delta]].

### Remark

For each of these integrals the case $m = n = 0$ can easily be done separately. We include these cases in the calculations set out below that prove the lemma.

### Proof
The proof is direct, using the trigonometric identities above.

If $n\neq m$ then    
    
$$
\begin{align*}
\int_{-\pi}^{\pi} \sin(nx)\cos (mx) \rd x
&= \int_{-\pi}^{\pi} \frac {1}{2} \Big[
	\sin ((n-m)x) + \sin ((n+m)x)
\Big] \rd x, \\
&= \frac {1}{2}\left[
	-\frac{\cos((n-m)x)}{n-m} -\frac{\cos ((n+m)x)}{n+m}
\right ]_{-\pi }^{\pi }, \\
&= 0.
\end{align*}
$$
^eq-11-11

If $n=m$ the proof is similar, with the first term disappearing since $\sin (0 \cdot x)=0$, and the answer is zero again.
    
*   2. If $n\neq m$ then
    
    
$$ \begin{align*} \int _{-\pi }^{\pi }\cos (nx)\ \cos (mx)\, \mathrm {d}x &= \int _{-\pi }^{\pi } \frac {1}{2}\Big [\cos ((n-m)x) +\cos ((n+m)x)\Big ]\, \mathrm {d}x,\\ &= \frac {1}{2}\left [\frac {\sin ((n-m)x) }{n-m}+ \frac {\sin ((n+m)x)}{n+m}\right ]_{-\pi }^{\pi },\\ &= 0. \end{align*} $$
^eq-11-11
 If $n=m\neq 0$ then
    
    
$$ \begin{align*} \int _{-\pi }^{\pi } \cos (nx)\ \cos (mx)\, \mathrm {d}x &= \int _{-\pi }^{\pi } \frac {1}{2}\Big [\cos (0x)+\cos (2m x) \Big ]\, \mathrm {d}x,\\ &= \frac {1}{2}\left [x+\frac {\sin (2m x)}{2m}\right ]_{-\pi }^{\pi },\\ &= \pi . \end{align*} $$
^eq-11-11
 If $n=m=0$
    
    
$$ \begin{align*} \int _{-\pi }^{\pi } \cos (nx)\ \cos (mx)\, \mathrm {d}x &= \int _{-\pi }^{\pi } 1\cdot 1\, \rd x,\\ &= 2\pi . \end{align*} $$
^eq-11-11

    
*   3) If $m\neq n$
    
    
$$ \begin{align*} \int _{-\pi }^{\pi } \sin (nx)\ \sin (mx)\, \mathrm {d}x &= \int _{-\pi }^{\pi } \frac {1}{2}\Big [-\cos ((n+m)x) +\cos ((n-m)x)\Big ]\, \mathrm {d}x,\\ &= \frac {1}{2}\left [-\frac {\sin ((n+m)x)}{n+m}+\frac {\sin ((n-m)x)}{n-m} \right ]_{-\pi }^{\pi },\\ &= 0. \end{align*} $$
^eq-11-11
 If $m=n\neq 0$
    
    
$$ \begin{align*} \int _{-\pi }^{\pi }\sin (nx)\sin (mx)\, \mathrm {d}x & =\int _{-\pi }^{\pi }\frac {1}{2}\Big [-\cos ((2m)x)+\cos ((0)x)\Big ]\, \mathrm {d}x,\\ & =\frac {1}{2}\left [-\frac {\sin (2mx)}{2m}+x\right ]_{-\pi }^{\pi },\\ & =\pi . \end{align*} $$
^eq-11-11
 Finally, if $m=n=0$ then the integrand is zero and so the value for the integral is zero as well.
    

### Remark
Why is this called an ‘orthogonality lemma’ ? Although a full discussion is beyond the scope of this unit, if we consider that the operation of integrating the product of two functions is in some sense like a scalar product on functions (i.e. a binary operation that results in a single real number) then the orthogonality lemma shows that the functions $1$, $\sin {x}$, $\cos {x}$, $\sin {2x}$, $\cos 2x, \ldots$ are orthogonal to each other with respect to this scalar product (also sometimes called an ‘inner product’). Thus a sum of sines or cosines with coefficients is rather like a linear combination of basis vectors multiplied by coefficients, i.e. an element of a vector space. Indeed these Fourier series appear to have an ‘infinite-dimensional vector space’ structure and the sines and cosines form an orthogonal basis for $2\pi$-periodic functions.

## 11.7 Orthogonality Lemma

Let $n,m \in \Z \setminus 0$. Then the following results hold:

$$
\begin{align}
\int_{-\pi }^{\pi }\sin (nx)\cos (mx)\, \mathrm {d}x &= 0,  \\
\int _{-\pi }^{\pi }\cos (nx)\ \cos (mx)\, \mathrm {d}x &= \pi \delta _{mn},  \\
\int _{-\pi }^{\pi }\sin (nx)\ \sin (mx)\, \mathrm {d}x &= \pi \delta _{mn},  \end{align} $$
^eq-11-100

where $\delta$ is the [[Kronecker Delta]].

### Remark

For each of these integrals the case $m = n = 0$ can easily be done separately. We include these cases in the calculations set out below that prove the lemma.

### Proof

The proof is direct, using the trigonometric identities above.

If $n\neq m$ then    
    
$$
\begin{align*}
\int_{-\pi}^{\pi} \sin(nx)\cos (mx) \rd x
&= \int_{-\pi}^{\pi} \frac {1}{2} \Big[
	\sin ((n-m)x) + \sin ((n+m)x)
\Big] \rd x, \\
&= \frac {1}{2}\left[
	-\frac{\cos((n-m)x)}{n-m} -\frac{\cos ((n+m)x)}{n+m}
\right ]_{-\pi }^{\pi }, \\
&= 0.
\end{align*}
$$
^eq-11-11

If $n=m$ the proof is similar, with the first term disappearing since $\sin (0 \cdot x)=0$, and the answer is zero again.
    
If $n\neq m$ then
    
    
$$ \begin{align*} \int _{-\pi }^{\pi }\cos (nx)\ \cos (mx)\, \mathrm {d}x &= \int _{-\pi }^{\pi } \frac {1}{2}\Big [\cos ((n-m)x) +\cos ((n+m)x)\Big ]\, \mathrm {d}x,\\ &= \frac {1}{2}\left [\frac {\sin ((n-m)x) }{n-m}+ \frac {\sin ((n+m)x)}{n+m}\right ]_{-\pi }^{\pi },\\ &= 0. \end{align*} $$
^eq-11-11

If $n=m\neq 0$ then
    
    
$$ \begin{align*} \int _{-\pi }^{\pi } \cos (nx)\ \cos (mx)\, \mathrm {d}x &= \int _{-\pi }^{\pi } \frac {1}{2}\Big [\cos (0x)+\cos (2m x) \Big ]\, \mathrm {d}x,\\ &= \frac {1}{2}\left [x+\frac {\sin (2m x)}{2m}\right ]_{-\pi }^{\pi },\\ &= \pi . \end{align*} $$
^eq-11-11

 If $n=m=0$
    
    
$$ \begin{align*} \int _{-\pi }^{\pi } \cos (nx)\ \cos (mx)\, \mathrm {d}x &= \int _{-\pi }^{\pi } 1\cdot 1\, \rd x,\\ &= 2\pi . \end{align*} $$
^eq-11-11

    
*   3) If $m\neq n$
    
    
$$ \begin{align*} \int _{-\pi }^{\pi } \sin (nx)\ \sin (mx)\, \mathrm {d}x &= \int _{-\pi }^{\pi } \frac {1}{2}\Big [-\cos ((n+m)x) +\cos ((n-m)x)\Big ]\, \mathrm {d}x,\\ &= \frac {1}{2}\left [-\frac {\sin ((n+m)x)}{n+m}+\frac {\sin ((n-m)x)}{n-m} \right ]_{-\pi }^{\pi },\\ &= 0. \end{align*} $$
^eq-11-11
 If $m=n\neq 0$
    
    
$$ \begin{align*} \int _{-\pi }^{\pi }\sin (nx)\sin (mx)\, \mathrm {d}x & =\int _{-\pi }^{\pi }\frac {1}{2}\Big [-\cos ((2m)x)+\cos ((0)x)\Big ]\, \mathrm {d}x,\\ & =\frac {1}{2}\left [-\frac {\sin (2mx)}{2m}+x\right ]_{-\pi }^{\pi },\\ & =\pi . \end{align*} $$
^eq-11-11
 Finally, if $m=n=0$ then the integrand is zero and so the value for the integral is zero as well.
    

### Remark
Why is this called an ‘orthogonality lemma’ ? Although a full discussion is beyond the scope of this unit, if we consider that the operation of integrating the product of two functions is in some sense like a scalar product on functions (i.e. a binary operation that results in a single real number) then the orthogonality lemma shows that the functions $1$, $\sin {x}$, $\cos {x}$, $\sin {2x}$, $\cos 2x, \ldots$ are orthogonal to each other with respect to this scalar product (also sometimes called an ‘inner product’). Thus a sum of sines or cosines with coefficients is rather like a linear combination of basis vectors multiplied by coefficients, i.e. an element of a vector space. Indeed these Fourier series appear to have an ‘infinite-dimensional vector space’ structure and the sines and cosines form an orthogonal basis for $2\pi$-periodic functions.