# 2.2 Derivatives of basic functions

## Theorem 2.7

Let $n \in \N$ and $p: \R \to \R$ be given by

$$
p(x) = \sum _{k=0}^n a_k x^k ,
$$

where $a_0,\ldots ,a_n\in \R$. Then for any $c\in \R$, $p$ is differentiable at $c$, and

$$
p^\prime (c) = \sum ^{n}_{k=1} k a_k c^{k-1}.
$$

### Proof

We first prove that monomials are differentiable. A monomial $m:\R \to \R$ is a function of the form

$$
m(x) = x^n
$$

where $n\in \N$. Let $c\in \R$. Then

%%\seteqnumber{0}{2.}{1}%%

$$
\begin{align*} \lim _{h\to 0}\frac {m(c+h)-m(c)}{h} &= \lim _{h\to 0}\frac {(c+h)^n-c^n}{h} \\ & =\lim _{h\to 0} \sum _{k=1}^n \binom {n}{k} c^{n-k} h^{k-1} \\ &= n c^{-1} . \end{align*}
$$

This shows that $m$ is differentiable at $c$ and $m’(c) = n c^{n-1}$.

Then the differentiability of a polynomial follows from the algebra for derivatives, Theorem 2.5. □

## Theorem 2.8

The functions $\exp$, $\sin$, $\cos$ defined in (1.8) are differentiable in $\R$ and

%%\seteqnumber{0}{2.}{1}%%

$$
\begin{align*} \exp ’(x) = \exp (x) , \quad \sin ’(x)=\cos (x), \quad \cos ’(x) = -\sin (x). \end{align*}
$$

### Proof

First we prove that $\exp$ is differentiable at $c=0$. For this we derive first the following inequality:

%%\seteqnumber{0}{2.}{1}%%

$$
\begin{align} \Bigl | \frac {\exp (x)-1}{x} -1 \Bigr | \leq e |x| , \quad \forall x\in [-1,1] , \end{align}
$$

where $e = \exp (1)$. Indeed, we start by observing that

%%\seteqnumber{0}{2.}{2}%%

$$
\begin{align*} \exp (x) -1 &= \sum _{k=1}^\infty \frac {x^k}{k!} = x \sum _{k=0}^\infty \frac {x^k}{(k+1)!} \end{align*}
$$

and

%%\seteqnumber{0}{2.}{2}%%

$$
\begin{align*} \frac {\exp (x)-1}{x} -1 &= \sum _{k=1}^\infty \frac {x^k}{(k+1)!} = x \sum _{k=0}^\infty \frac {x^k}{(k+2)!} \end{align*}
$$

For $x\in [-1,1]$,

%%\seteqnumber{0}{2.}{2}%%

$$
\begin{align*} \left | \sum _{k=0}^\infty \frac {x^k}{(k+2)!} \right | & \leq \sum _{k=0}^\infty \frac {1}{k ! } = e . \end{align*}
$$

and this proves (2.2). From (2.2) we deduce that

%%\seteqnumber{0}{2.}{2}%%

$$
\begin{align*} \lim _{h\to 0} \Bigl [ \frac {\exp (h)-1}{h} -1 \Bigr ]=0 \end{align*}
$$

which is the same as

$$
\lim _{h\to 0} \frac {\exp (h)-1}{h} = 1.
$$

Therefore $\exp$ is differentiable at $0$ and $\exp ’(0)=1$.

Let us prove that $\exp$ is differentiable at $c\in \R$. For this recall that $\exp (x+y) = \exp (x) \exp (y)$ for all $x,y\in \R$ and therefore

%%\seteqnumber{0}{2.}{2}%%

$$
\begin{align*} \lim _{h\to 0}\frac {\exp (c+h)-\exp (c)}{h} &= \lim _{h\to 0}\frac {\exp (c)\exp (h)-\exp (c)}{h} \\ & = \exp (c) \lim _{h\to 0}\frac {\exp (h)-\exp (0)}{h} =\exp (c). \end{align*}
$$

This shows that $\exp$ is differentiable at $c\in \R$ and $\exp ’(c) = \exp (c)$.

The proof for $\sin$ and $\cos$ are similar. We only prove the relevant inequality

%%\seteqnumber{0}{2.}{2}%%

$$
\begin{align*} \Bigl | \frac {\sin (x)}{x}-1\Bigr | \leq e x^2 , \quad |x|\leq 1. \end{align*}
$$

Indeed, for $|x|\leq 1$, we have

%%\seteqnumber{0}{2.}{2}%%

$$
\begin{align*} \Bigl | \frac {\sin (x)}{x}-1\Bigr | &= \Bigl | \sum _{n=0}^\infty (-1)^n \frac {x^{2n}}{(2n+1)!}-1 \Bigr | \\ &= \Bigl | \sum _{n=1}^\infty (-1)^n \frac {x^{2n}}{(2n+1)!} \Bigr | \\ & \leq x^2 \sum _{n=1}^\infty \frac {1}{(2n+1)!} \\ & \leq x^2 \sum _{n=0}^\infty \frac {1}{n!} \\ & \leq e x^2. \end{align*}
$$

□
