# 2.6 Higher order derivatives

## Definition 2.34

Let $a<b$, $f \colon (a,b) \to \R$ and $c\in (a,b)$. We say that $f$ is twice differentiable at $c$ if there exists $\delta >0$ such that $(c-\delta , c+\delta )\subset (a,b)$, $f$ is differentiable in $(c-\delta , c+\delta )$ and $f’\colon (c-\delta , c+\delta )\to \R$ is differentiable at $c$.

We call $(f^\prime )^\prime (c)$ the _second derivative_ of $f$ at $c$, written $f^{\prime \prime }(c)$ or $f^{(2)}(c)$. We say that $f$ is twice differentiable on $(a,b)$ if it is twice differentiable at every point in $(a,b)$.

## Definition 2.35

Let $n\in \N$. We define the notion that $f \colon (a,b) \to \R$ is $n$-times differentiable at $c\in (a,b)$ recursively as follows. For $n=1$ and $n=2$ this was already done. If $n\geq 3$, we say that $f$ is $n$-times differentiable at $c\in (a,b)$ if there is $\delta >0$ such that $(c-\delta , c+\delta )\subset (a,b)$, $f$ is $(n-1)$-times differentiable in $(c-\delta , c+\delta )$ and $f^{(n-1)}\colon (c-\delta , c+\delta )\to \R$ is differentiable at $c$. The $n$-th derivative of $f$ at $c$ is defined as $(f^{(n-1)})’(c)$ and denoted by $f^{(n)}(c)$.

### Example 2.36

.

Polynomials, the exponential function, and the trigonometric functions are $n$-times differentiable for all $n\in \N$.

### Example 2.37

.

Let $f \colon \R \rightarrow \R$, be given by

$$
f(x) := \left \{\begin {array}{rll} x^2, &\quad &x \geq 0.\\ -x^2, & & x < 0.\end {array}\right .
$$

We see that

%%\seteqnumber{0}{2.}{5}%%

$$
f^\prime (c) = 2c \text { for } c>0 , , \qquad f^\prime (c)= -2c \text { for } c<0.
$$

(by Theorem 2.7). For $c=0$,

$$
\frac {f(0+h) - f(0)}{h} = \left \{\begin {array}{rll} h, & \quad &h > 0,\\ -h, & & h < 0, \end {array}\right .
$$

and this implies,

$$
\lim _{h\to 0}\frac {f(0+h)-f(0)}{h} = 0.
$$

Thus, $f^\prime \colon \R \rightarrow \R$ is given $f^\prime (x) = 2|x|$. By Example 2.4, $f^\prime$ is _not_ differentiable at $c=0$. But

$$
f^{\prime \prime }(c) = \left \{\begin {array}{rll} 2, & \quad &c > 0,\\ -2, &\quad & c < 0.\end {array}\right .
$$

— $\circ$ —

Higher order derivatives appear naturally when trying to gain a better understanding of the limit that defines the derivative

%%\seteqnumber{0}{2.}{5}%%

$$
f’(c) = \lim _{x\to c} \frac {f(x)-f(c)}{x-c}.
$$

Recall that the existence of this limit is equivalent to say that there exists a number $f’(c)$ such that

%%\seteqnumber{0}{2.}{5}%%

$$
\lim _{x\to c} \frac {f(x)-f(c)-f’(c)(x-c)}{x-c} = 0.
$$

This means that, if we define

%%\seteqnumber{0}{2.}{5}%%

$$
R(x)= f(x)-f(c)-f’(c)(x-c)
$$

so that

%%\seteqnumber{0}{2.}{5}%%

$$
\label {eqR} f(x) = f(c) + f’(c)(x-c) + R(x),
$$

then

%%\seteqnumber{0}{2.}{6}%%

$$
\lim _{x\to c} \frac {R(x)}{x-c} = 0.
$$

This limit can be interpreted as saying that the remainder $R$ in equation (2.6) is much smaller that $x-c$ when $x\to c$. But can we get a more precise description of $R(x)$? Let us proceed assuming that $f$ has all the necessary derivatives, and let us apply De l’Hospital’s Rule, Theorem 2.32. We get that

%%\seteqnumber{0}{2.}{6}%%

$$
\begin{aligned} \lim _{x\to c} \frac {R(x)}{(x-c)^2} &= \lim _{x\to c} \frac {f(x)-f(c)-f’(c)(x-c)}{(x-c)^2} \\ &= \lim \_{x\to c} \frac {f’(x)-f’(c)}{2(x-c)} \\ &= \frac {1}{2} f^{\prime \prime }(c) . \end {aligned}
$$

We then deduce that

%%\seteqnumber{0}{2.}{6}%%

$$
R(x) \approx \frac {1}{2}f^{\prime \prime }(c) (x-c)^2,
$$

when $x$ is close to $c$. This formula says with more precision how much smaller is $R(x)$ compared to $x-c$, and also allows us to write

%%\seteqnumber{0}{2.}{6}%%

$$
f(x) \approx f(c) + f’(c)(x-c) + \frac {1}{2} f^{\prime \prime }(c) (x-c)^2,
$$

when $x$ is close to $c$. However, there is still an imprecision when we use the symbol $\approx$. Taylor’s theorem below gives a rigorous description of $R(x)$ and generalises the previous discussion to higher order derivatives.

Theorem 2.38 (Taylor’s theorem).

Let $n\in \N$, $a<b$ and $f\colon (a,b) \to \R$ be $(n+1)$-times differentiable in $(a,b)$. Let $x_0 \in (a,b)$. Then for $x\in (a,b)$,

$$
f(x) = f(x_0) + f’(x_0)(x-x_0) + \frac {1}{2}f^{\prime \prime }(x_0)(x-x_0)^2 + \ldots + \frac {1}{n!} f^{(n)}(x_0)(x-x_0)^n + R_n(x)
$$

where

%%\seteqnumber{0}{2.}{6}%%

$$
\begin{align} \label {formula Rn} R_n(x) = \frac {1}{(n+1)!} f^{(n+1)}(c)(x-x_0)^{n+1} , \end{align}
$$

and $c \in (x_0,x)$ if $x>x_0$ and $c \in (x,x_0)$ if $x<x_0$.

### Proof
 The function $R_n(x)$ is defined by

$$
R*n(x) = f(x) - \sum *{j=0}^n \frac {f^{(j)}(x_0)}{j!} (x-x_0)^j, \quad x \in (a,b)
$$

and we see that it is $(n+1)$-differentiable in $(a,b)$.

We claim that

$$
R_n^{(k)}(x_0) = 0, \quad k=0,\ldots ,n.
$$

Indeed,

$$
R_n(x_0) = 0
$$

and

%%\seteqnumber{0}{2.}{7}%%

$$
\begin{align*} R*n’(x) &= f’(x) - \sum *{j=1}^n \frac {f^{(j)}(x_0)}{(j-1)!} (x-x_0)^{j-1} , \\ R_n’(x_0) &= f’(x_0) - f’(x_0) =0. \end{align*}
$$

Inductively, for any $k=0,\ldots ,n$,

%%\seteqnumber{0}{2.}{7}%%

$$
\begin{align*} R*n^{(k)}(x) &= f^{(k)}(x) - \sum *{j=k}^n \frac {f^{(j)}(x_0)}{(j-k)!} (x-x_0)^{j-k} , \\ R_n^{(k)}(x_0) &= f^{(k)}(x_0) - f^{(k)}(x_0) =0. \end{align*}
$$

We observe that

$$
R_n^{(n+1)}(x) = f^{(n+1)}(x).
$$

Let us prove the formula for $R_n(x)$ when $x\in (a,b)$ and $x>x_0$. By the Cauchy mean value theorem, Theorem 2.24,

%%\seteqnumber{0}{2.}{7}%%

$$
\begin{align*} \frac {R_n(x)}{(x-x_0)^{n+1}} = \frac {R_n’(c_1)}{(n+1)(c_1-x_0)^n} \end{align*}
$$

for some $x_0<c_1<x$. (Observe that both the numerator and denominator of the left hand side are zero when evaluated at $x_0$.) Again, by the Cauchy mean value theorem, there is $x_0<c_2<c_1$ such that

%%\seteqnumber{0}{2.}{7}%%

$$
\begin{align*} \frac {R_n’(c_1)}{(n+1)(c_1-x_0)^n} = \frac {R_n^{\prime \prime }(c_2)}{(n+1)n(c_2-x_0)^{n-1}} . \end{align*}
$$

(Here we consider the right hand side as a function of $c_1$.) Inductively, there are $x_0<c_k<c_{k-1}$ such that

%%\seteqnumber{0}{2.}{7}%%

$$
\begin{align*} \frac {R*n(x)}{(x-x_0)^{n+1}} &= \frac {R_n^{k-1}(c*{k-1})}{(n+1)\cdot \ldots \cdot (n-k+3) (c\_{k-1}-x_0)^{n-k+2}} \\ &= \frac {R_n^{k}(c_k)}{(n+1)\cdot \ldots \cdot (n-k+2) (c_k-x_0)^{n-k+1}} \end{align*}
$$

for $k=1,\ldots ,n$. For $k=n$ this formula gives

%%\seteqnumber{0}{2.}{7}%%

$$
\begin{align*} \frac {R_n(x)}{(x-x_0)^{n+1}} = \frac {R_n^{(n)}(c_n) }{(n+1)! (c_n-x_0)} \end{align*}
$$

Applying once more the Cauchy mean value theorem, we find $x_0<c<c_{n}<\ldots <x$ such that

%%\seteqnumber{0}{2.}{7}%%

$$
\begin{align*} \frac {R_n(x)}{(x-x_0)^{n+1}} = \frac {f^{(n+1)}(c) }{(n+1)! }, \end{align*}
$$

which is the same as (2.7).

□

### Example 2.39

.

Apply Taylor’s Theorem to rigorously approximate $e=\exp (1)$ to an accuracy of $10^{-2}$.

### Solution

.

Let $f(x)=\exp (x)$. We know that $f^{(n)}(0)=1$ for all $n\in \N \cup \{0\}$. Let $n\in \N$. By Taylor’s Theorem, there is $c\in (0,\,1)$ such that, for $\displaystyle \Sigma _n:=\sum _{k=0}^{n}\frac {1}{k!}$,

$$
\exp (1)-\Sigma \_n=R_n=\frac {f^{(n+1)}(c)}{(n+1)!}.
$$

Now, $f^{(n+1)}(x)=\exp (x)$, which is increasing. Thus, $f^{(n+1)}(c)\leq \exp (1)$, which means that

$$
0\leq \exp (1)-\Sigma \_n \leq \frac {\exp (1)}{(n+1)!}.
$$

Hence,

$$
\exp (1)<\frac {\Sigma \_n}{1-\frac {1}{(n+1)!}}
$$

Therefore

$$
\left |\exp (1)-\Sigma \_n\right |=|R_n|=\frac {f^{(n+1)}(c)}{(n+1)!}\leq \frac {\exp (1)}{(n+1)!}\leq \frac {\Sigma \_n}{(n+1)!-1}.
$$

Let $d_n = \frac {\Sigma _n}{(n+1)!-1}$. We compute

%%\seteqnumber{0}{2.}{7}%%

$$
\begin{matrix} n=1, & \Sigma _n =2 , & d_n=2 \\ n=2 , &\Sigma _n =2.5 , & d_n=0.5 \\ n=3, &\Sigma _n = 2.66666666667, &d_n=0.116 \\ n=4, &\Sigma _n = 2.70833333333, &d_n=0.0228 \\ n=5, &\Sigma _n = 2.71666666667, & d_n=0.00378<10^{-2} \end {matrix}
$$

and therefore $|\exp (1) - \Sigma _5|<10^{-2}$.
