## Contrapositive

Given two statements $P$ and $Q$ , the implication

$$
P \implies Q
$$

is equivalent to

$$
\neg  Q \implies \neg  P
$$

### Proof

We already know that the implication $P \implies Q$ is equivalent to $(\neg  P ) \lor Q$ , which in turn may be written in the form $Q \lor (\neg  P )$ . Now we observe that $Q \iff \neg  (\neg  Q )$ , and therefore, we conclude that $Q \lor (\neg  P )$ is equivalent to $\neg  (\neg  Q ) \lor (\neg  P )$ . Finally, the last statement can be written in the form $\neg  Q \implies \neg  P$ . â–¡
