[[next](MA10210se17.html)] [[tail](#tailMA10210se16.html)] [[up](MA10210ch4.html#MA10210se16.html)]

### 4.1 [Sum formula](MA10210.html#QQ2-22-35)

Definition 1.  
For a matrix $A\in M_{n \times n}\left( \F \right)$

$$
\begin{align}
 \det A=\underset{\sigma \in S_{n}}{\sum}\left( sgn \sigma \right)a_{\sigma \left( 1 \right) 1}\dots a_{\sigma \left( n \right) n} & & & \text{(1)}\text{}\text{}
\end{align}
$$

where $S_{n}$ is the symmetric group of self-bijections of $\left\{ 1 , \dots  , n \right\}$ and  
$\left( sgn \sigma \right)\in\left\{ + 1 , - 1 \right\}$ is the sign homomorphism.

Note: there are $n!$ many terms in the sum formula, the amount of work for computing $ \det $ following the definition is large if $n$ is big. In this chapter we will discuss various properties of $ \det $ and how to apply them to compute $ \det $ . We also write the determinant $ \det A$ as $\left|A\left|$.

Example 2.  

1.

$n=2$ 
$$
\begin{align}
 \det \begin{pmatrix} \begin{matrix}a_{1 1} & a_{1 2} \\ a_{2 1} & a_{2 2}\end{matrix} \end{pmatrix} & = & \begin{vmatrix} \begin{matrix}a_{1 1} & a_{1 2} \\ a_{2 1} & a_{2 2}\end{matrix} \end{vmatrix} & \text{} \\ & = & a_{1 1}a_{2 2}-a_{2 1}a_{1 2} & \text{}
\end{align}
$$

2.

$n=3$

$$
\begin{align}
 & &  \det \begin{pmatrix} \begin{matrix}a_{1 1} & a_{1 2} & a_{1 3} \\ a_{2 1} & a_{2 2} & a_{2 3} \\ a_{3 1} & a_{3 2} & a_{3 3}\end{matrix} \end{pmatrix} & \text{} \\ & = & a_{1 1}a_{2 2}a_{3 3}+a_{1 2}a_{2 3}a_{3 1}+a_{1 3}a_{2 1}a_{3 2} & \text{} \\ & & -a_{1 1}a_{3 2}a_{2 3}-a_{2 1}a_{1 2}a_{3 3}-a_{3 1}a_{2 2}a_{1 3} & \text{}
\end{align}
$$

3.

Identity matrix

$$
 \det  \left( I \right) = 1
$$

as all summands are $0$ except $\sigma=id$ (so that $\sigma\left( j \right)=j\forall j$ ) then $sgn\sigma=1$ and all factors $=1$ .

4.

Upper triangular matrices:

$$
\begin{align}
A = \begin{pmatrix} a_{1 1} & & * \\ & \ddots & \\ 0 & & a_{n n} \end{pmatrix}
\end{align}
$$

has $ \det A=a_{1 1}\dots a_{n n}$ as all summands are $0$ unless

$$
\begin{align}
 & & \sigma\left( j \right)\leq j\forall j & \text{} \\ & \Rightarrow & \sigma\left( 1 \right)=1,\sigma\left( 2 \right)=2,\dots  & \text{} \\ & \Rightarrow & \sigma=id. & \text{}
\end{align}
$$

5.

Lower triangular matrices:

$$
\begin{align}
A = \begin{pmatrix} a_{1 1} & & 0 \\ & \ddots & \\ * & & a_{n n} \end{pmatrix}
\end{align}
$$

Similar to upper triangular matrices, $ \det A=a_{1 1}\dots a_{n n}$ .

Proposition 3.  
If

$$
\begin{align}
A = \begin{pmatrix} A^{′} & * \\ 0 & A^{''} \end{pmatrix}
\end{align}
$$

( $A^{′}\in M_{k , k}$ and $A^{′}\in M_{l , l}$ ) is ‘blockwise upper triangular’, then

$$
 \det  A =  \det  A^{′} \cdot  \det  A^{''} .
$$

Proof. The summands in the formula are zero unless $\sigma\left( i \right)\leq k$ for all $i\leq k$ , so that $\sigma$ permutes $\left\{ 1 , \dots  , k \right\}$ and $\left\{ k + 1 , \dots  , k + l \right\}$ separately. Further, any such ‘split’ permutation can occur. Denote the symmetric groups of $\left\{ 1 , \dots  , k \right\}$ and $\left\{ k + 1 , \dots  , k + l \right\}$ by $S_{k}$ and $S_{l}$ , respectively. Writing

$$
\sigma = \left( \left(\sigma\right)^{′} , \left(\sigma\right)^{''} \right) \in S_{k} \times S_{l} ,
$$

we have $sgn\sigma=sgn\left(\sigma\right)^{′}\cdot sgn\left(\sigma\right)^{''}$ and

$$
\begin{align}
 &  \det A & & \\ & =\left(\underset{\left(\sigma\right)^{′} \in S_{k}}{\sum} \left( sgn \left(\sigma\right)^{′} \right) a_{\left(\sigma\right)^{′} \left( 1 \right) 1} \dots  a_{\left(\sigma\right)^{′} \left( k \right) k}\right)\cdot\left(\underset{\left(\sigma\right)^{''} \in S_{l}}{\sum} \left( sgn \left(\sigma\right)^{''} \right) a_{\left(\sigma\right)^{''} \left( k + 1 \right) , k + 1} \dots  a_{\left(\sigma\right)^{''} \left( k + l \right) , k + l}\right) & & \\ & = \det A^{′}\cdot \det A^{''}. & \square
\end{align}
$$

Note.  
Repeated applications give a similar formula for $n$ -block upper (and lower) triangular matrices.

Proposition 4.  

$$
 \det  A^{T} =  \det  A .
$$

Proof. Let $A=\left( a_{i j} \right)$ . Then $A^{T}=\left( \left(\overset{̃}{a}\right)_{i j} \right)$ with $\left(\overset{̃}{a}\right)_{i j}=a_{j i}$ . We have

$$
\begin{align}
 \det A^{T} & = & \underset{\sigma \in S_{n}}{\sum}\left( sgn \sigma \right)\left(\overset{̃}{a}\right)_{\sigma \left( 1 \right) 1}\dots \left(\overset{̃}{a}\right)_{\sigma \left( n \right) n} & \text{} \\ & = & \underset{\sigma \in S_{n}}{\sum}\left( sgn \sigma \right)a_{1 \sigma \left( 1 \right)}\dots a_{n \sigma \left( n \right)} & \text{} \\ & = & \underset{\tau \in S_{n}}{\sum}\left( sgn \left(\tau\right)^{- 1} \right)a_{\tau \left( 1 \right) 1}\dots a_{\tau \left( n \right) n}\tau=\left(\sigma\right)^{- 1} & \text{}
\end{align}
$$

where product is rearranged into column index order. The summation range is same because $\sigma\rightarrow tail\left(\sigma\right)^{- 1}$ is a bijection $S_{n}\rightarrow S_{n}$ .

Also,

$$
\begin{align}
sgn\left( \left(\tau\right)^{- 1} \right)sgn\left( \tau \right) & = & sgn\left( \left(\tau\right)^{- 1} \tau \right) & \text{} \\ & = & sgn\left( id \right) & \text{} \\ & = & 1 & \text{}
\end{align}
$$

and so

$$
sgn \left( \left(\tau\right)^{- 1} \right) = \frac{1}{sgn \left( \tau \right)} = sgn \left( \tau \right)
$$

as $sgn=\pm1$ .

Hence $ \det A^{T}= \det A$ , as required. □

[[next](MA10210se17.html)] [[front](MA10210se16.html)] [[up](MA10210ch4.html#MA10210se16.html)]