# Solving the Wave Equation

The Wave Equation is a PDE over a function $u(x, t) : \R \times \R \to \R$ where,

$$
u_{tt} = c^2 u_{xx},
$$

^wave-equation

This equation models, among other things, small amplitude[^1] transverse vibrations of a finite length string, $x \in [0, L]$. In this case $u(x, t)$ corresponds to the transverse position of the string, and where $c = \sqrt{\frac T\rho}$ is known as the wave speed, and depends on the tension, $T$, and density $\rho$ in the string.

[^1]: Why? Discuss physics of this.

## Boundary Conditions

The traditional boundary conditions for the Wave Equation on a string come in two varieties, fixed and non-fixed ends.

### Fixed Ends

Given an initial displacement $u_0(x)$ and initial velocity $v_0(x)$ we have a problem defined as so,

- Wave Equation $u_{tt} = c^2 u_{xx}$
- Fixed Ends (Boundary Conditions): $0 = u(0, t) \land 0 = u(L, t)$
- Initial Conditions
	- $u(x, 0) = u_0(x)$
	- $u_t(x, 0) = v_0(x)$

^fixed-ends-bvp

Fixed ends is a [[14.22 Dirichlet Boundary Condition|Dirichlet Boundary Condition]].

### Mobile Ends

Given the same initial displacement $u_0(x)$ and velocity $v_0(x)$, but with the Mobile Ends Boundary Condition,

- Wave Equation $u_{tt} = c^2 u_{xx}$
- Mobile Ends (Boundary Conditions): $0 = u_x(0, t) \land 0 = u_x(L, t)$
- Initial Conditions
	- $u(x, 0) = u_0(x)$
	- $u_t(x, 0) = v_0(x)$

Mobile ends is a [[14.23 Neumann boundary condition|Neumann Boundary Condition]].

> #todo find an example image of these two

## Solving the [[#Fixed Ends]] / [[14.22 Dirichlet Boundary Condition|Dirichlet Problem]] Wave Equation

Solving the [[#Fixed Ends]] problem above, we first assume [[Separation of Variables]], proposing a trail solution,

$$
u(x,t) = X(x) G(t).
$$

^eq-16-3

Substituting this into the [[#^wave-equation|Wave Equation]] above we get,

$$
X(x) G''(t) = c^2 X''(x) G(t)
$$

which after a bit of rearranging becomes,

$$
\frac{G''(t)}{G(t)} = c^2 \frac{X''(x)}{X(x)}.
$$

Applying similar logic to that seen in our [[10.4 Motivation for Fourier Series from Heat Equation|solution to the Heat Equation]] we can deduce that the disjoint parameters of two implies that they are both constant and thus:

$$
\begin{align}
- \lambda ^2 &= \frac{G''(t)}{G(t)} \\
- \lambda ^2 &= c^2 \frac{X''(x)}{X(x)}.
\end{align}
$$

As for the heat equation, we know this constant must be negative, but this can really only be justified [[a posteriori]] by investigating the alternative cases as determining that no solutions are available that satisfy the boundary conditions.

This gives us two separate ODEs for $X$ and $G$,

$$ 
\begin{align}
0 &= G''(t) + \lambda ^2 G(t) \\
0 &= X''(x) + \(\frac{\lambda}{c}\)^2 X(x).
\end{align}
$$

with solutions,

$$
\begin{align}
G(t) &= A\cos(\lambda t) + B\sin(\lambda t) \\
X(x) &= C\cos\(\frac{\lambda}{c} x\) + D\sin\(\frac{\lambda}{c} x\) \\
\end{align}
$$

which can be plugged into to our original equation giving us,

$$
u(x, t) = \left[
	C\cos\(\frac{\lambda}{c} t\) 
	+ D\sin\(\frac{\lambda}{c} t\)
\right] \left[
	A\cos(\lambda t)
	+ B\sin(\lambda t)
\right].
$$

### Imposing Boundary Conditions

We can now impose the [[#Fixed Ends]] Boundary Conditions, after which we obtain,

$$
X(0)G(t) = X(L)G(t) = 0 \quad \Forall t > 0
$$

which by the [[Null Product Lemma]] leads to the conclusion that,

$$
X(0) = X(L) = 0.
$$

Computing the consequential coefficients we have,

$$
X(0) = 0 \implies C = 0
$$

and by this,

$$
\begin{align}
X(L)
&= 0\cos\(\frac{\lambda}{c} L\) + D\sin\(\frac{\lambda}{c} L\) \\
&= D\sin\(\frac{\lambda}{c} L\) \\
&= \sin\(\frac{\lambda}{c} L\) 
\implies \frac{\lambda}{c} L = \pi n, 
\quad n \in \Z
\end{align}
$$

which gives us $\lambda_n = \frac{n \pi c}{L}, n \in \Z$. Plugging these all back in gives the form,

$$
u(x,t) = D \sin\(\frac{n\pi}{L} x\) \left[
	A \cos\(\frac{n\pi c}{L} t\) + B \sin\(\frac{n\pi c}{L} t\)
\right],
\quad n\in \mathbb {Z}.
$$

which noting that $DA = A_n$ and $DB = B_n$ are arbitrary constants and hence,

$$
u(x,t) = \sin\(\frac{n\pi}{L} x\) \left[
	A_n \cos\(\frac{n\pi c}{L} t\) + B_n \sin\(\frac{n\pi c}{L} t\)
\right]
$$

^sol

for $n \ge 1$. This restriction on $n$ from $\Z$ to $n \ge 1$ comes from symmetry considerations where $i \equiv i$ under negation of $A_n$, and hence is not a linearly independent solution. Further $n = 0$ is the zero solution and thus redundant.

[[16.3 Example of Solving the Wave Equation]]

## Applying Initial Conditions

> #todo what are the different stages we go through here? How have we a solution then do again to develop it? General vs Particular? Null space of PDE? PDE vs BVP? Why have we only applied some of the conditions? Is it just because this is a Fourier and they want to separate it because we have just learned it?

Taking our [[#^sol|solution]] from above, we must now apply the initial conditions from above, ie that the initial position and velocity are given by $u_0(x)$ and $v_0(x)$,

$$
\begin{align}
u(x, 0) = u_0(x) \\
u_t(x, 0) = v_0(x).
\end{align}
$$

From the solution above we can compute the RHS of these equations to be,

$$
\begin{align}
u_n(x, 0) &= A_n \sin\(\frac{n\pi}{L} x\) \\
\frac{\p u_n}{\p t}(x, 0) &= \(\frac{n\pi c}{L}\) B_n \sin\(\frac{n\pi}{L} x\) \\
\end{align}
$$

which letting $b_n = \(\frac{n\pi c}{L}\) B_n$, gives us,

$$
\begin{align}
u_0(x) &= A_n \sin\(\frac{n\pi}{L} x\) \\
v_0(x) &= b_n \sin\(\frac{n\pi}{L} x\).
\end{align}
$$

which we we know we can solve using the [[12.8 Even and Odd Periodic Extensions|Odd Extension]] of $u_0$ and $v_0$ from $(0, L)$ to $(-L, L)$, and from there calculating the [[11.8 Fourier Coefficients|Fourier Coefficients]] in the usual manner (using [[11.8 Fourier Coefficients#Even and Odd Functions]] to restrict our domain to original $(0, L)$),

$$
\begin{align}
A_n &= \frac {2}{L} \int_{0}^{L}
	u_0(x)\sin\(\frac {n\pi x}{L}\)
\rd x. \\

b_n &= \frac {2}{L} \int_{0}^{L}
	v_0(x) \sin\(\frac{n\pi x}{L}\)
\rd x.
\end{align}
$$

> **Note** that this is an equation for $b_n$ **NOT** $B_n$, the conversion being:
> $$ B_n = \frac{L}{n\pi c} b_{n} $$

Thus giving us a solution to the full [[14.22 Dirichlet Boundary Condition|Dirichlet Boundary Problem]].

## Summary

Given the problem

![[#^fixed-ends-bvp]]

the expression is a solution

$$
u(x, t) = \sum_{n \in \N}
	\sin \(\frac{n\pi x}{L}\) \left[
		A_n \cos\(\frac{n\pi ct}{L}\) +
		B_n \sin\(\frac{n\pi ct}{L}\)
	\right]
$$

given

$$
\begin{align}
A_n &= \frac {2}{L} \int_{0}^{L}
	u_0(x)\sin\(\frac {n\pi x}{L}\)
\rd x. \\

B_n &= \frac {2}{L} \frac{L}{n\pi c} \int_{0}^{L}
	v_0(x) \sin\(\frac{n\pi x}{L}\)
\rd x.
\end{align}
$$
