# Square Wave Example FQQ

Find the Fourier series of the following function:

$$
\begin{gather}
f : [-\pi, \pi] \to \R \\\
f(x) = \begin {cases}
	-1 & -\pi \leq x < 0, \\
	\phantom {-}1 & 0 \leq x < \pi ,
\end {cases}
\end{gather}
$$

^62e778

under a [[11.2 Periodic Extension]] with period $2\pi$,

$$
f(x + 2\pi) = f(x).
$$

## Solution

Using definition [[12.7 Fourier Coefficients for General Periodic Function]] with $L=\pi$ we have

$$ a_0 = \frac {1}{\pi } \int _{-\pi }^{\pi } f(x) \, \mathrm {d}x = 0, $$

and


$$ \begin{align} a_n & = \frac {1}{\pi } \int _{-\pi }^{\pi } f(x) \cos (nx) \, \mathrm {d}x \\ &= \frac {1}{\pi } \int _{-\pi }^{0}(-1) \cos (nx) \, \mathrm {d}x +\frac {1}{\pi } \int _{0}^{\pi }(1) \cos (nx) \, \mathrm {d}x \\ &= -\frac {1}{\pi n} \big [\sin \left (nx\right )\big ]_{-\pi }^{0}+\frac {1}{\pi n}\ \big [\sin \left (nx\right )\big ]_{0}^{\pi } = 0. \end{align} $$

^eq-12-3

 Also,

$$ \begin{align*} b_n & = \frac {1}{\pi } \int _{-\pi }^{\pi } f(x) \sin (nx) \, \mathrm {d}x \\ & = \frac {1}{\pi } \int _{-\pi }^{0} (-1) \sin \left (nx\right )\, \mathrm {d}x + \frac {1}{\pi } \int _{0}^{\pi } (1) \sin \left (nx\right )\, \mathrm {d}x \\ & = \frac {1}{\pi n}\ \big [\cos \left (nx\right )\big ]_{-\pi }^{0} -\frac {1}{\pi n}\ \big [\cos \left (nx\right )\big ]_{0}^{\pi }. \end{align*} $$

^eq-12-6

 Remembering that $\cos n\pi = (-1)^n$, we see that


$$  \begin{aligned} b_n & = \frac {1}{\pi n}\Big ( 1 - (-1)^n\Big ) - \frac {1}{\pi n}\Big ((-1)^n - 1\Big ),\\ & = \frac {2}{\pi n}\Big ( 1 - (-1)^n\Big ), \end {aligned} $$

^eq-12-6

Hence


$$ \begin{aligned} b_n & = {\renewcommand {\baselinestretch }{1.5}\normalsize \begin{cases} \dfrac {4}{n\pi } & n\textrm { }\text {odd},\\ 0 & n\textrm { }\text {even}. \end {cases}} \end {aligned} $$

^eq-12-7

So we have computed a Fourier series representation

$$ f(x) = \lim _{N\to \infty } S_N(x) = \lim _{N\to \infty } \left [ \frac {4}{\pi }\sum _{n=1, \, \text {$n$ odd}}^N \frac {\sin \left (nx\right )}{n}\right ]. $$

^eq-12-8

## Remark

For Fourier series where half the coefficients vanish and the nonzero coefficients have either even or odd indices, it is common to rewrite the summation so that the index over which we sum increases in unit steps. Thus from [[#^eq-12-6]], we set $n = 2m + 1$ for $m = 0, 1, 2, \ldots$, so that


$$ b_{2m} = \frac {4}{(2m+1)\pi }. $$

^eq-12-9


The Fourier series can now be written as


$$  f(x) = \lim _{N\to \infty } S_N = \frac {4}{\pi } \sum _{m=0}^\infty \frac {\sin ([2m+1]x)}{2m+1}. $$

^eq-12-10