# Fourier Convergence Theorem

Let $f$ be a $2\pi$-[[11.1 Periodic Function|Periodic Function]], with $f(x)$ and $fâ€™(x)$ [[12.4 Piecewise Continuity|Piecewise Continuous]] on $(-\pi , \pi )$.

Then the [[Fourier Series]] of $f$ at $x$ **converges to the average of the left hand and right hand limits** (cf [[12.2 One-Sided Limits]]). That is,

$$
\frac {1}{2}\big [f(x_-) + f(x_+)\big ] = \frac {a_0}{2} + \sum _{n=1}^\infty [a_n\cos (nx) + b_n\sin (nx)]. $$

^eq-12-12

## Example

In the square-wave function

![[12.1 Square Wave Example FQQ#^62e778]]

with Fourier series

![[12.1 Square Wave Example FQQ#^eq-12-10]]

we have by the above theorem that at any point, $x$,

$$
\frac {1}{2}[f(x_-) + f(x_+)] = \frac {4}{\pi } \sum _{m=0}^\infty \frac {\sin [(2m+1)x]}{(2m+1)}.
$$

^eq-12-13


which agrees with the left hand limit at $x=0$ being $-1$ and the right hand limit at $x=0$ being $+1$, for example, so that both sides are zero.

Values of $x$ also lead to power series expansions for constants such as $\pi$. For example, evaluating the Fourier series at $x = \pi /2$ we have


$$ 1 = \frac {4}{\pi } \sum _{m=0}^\infty \frac {\sin [(2m+1)\frac {\pi }{2}]}{(2m+1)} = \frac {4}{\pi } \sum _{m=0}^\infty \frac {(-1)^m}{(2m+1)}, $$

^eq-12-14


and so we conclude that


$$ \sum _{m=0}^\infty \frac {(-1)^m}{(2m+1)} = \frac {\pi }{4} \, . $$

^eq-12-15