# Classification of Isolated Singularities

Let $z_0 \in \C$ and $r > 0$. Suppose that $f : B_r(z_0) \setminus \{z_0\} \to \C$ is holomorphic. Then the following holds true.

1.  The singularity at $z_0$ is a [[Removable Singularity]] if, and only if, there exists $s \in (0, r)$ such that $f$ is bounded in $B_s(z_0) \setminus \{z_0\}$. If so, then there exists a holomorphic function $g : B_r(z_0) \to \C$ such that $f(z) = g(z)$ for all $z \in B_r(z_0) \setminus \{z_0\}$. ^s1
	- Note the **change of domain** from $B_r(z_0) \setminus \set{z_0} \mapsto B_r(z_0)$.
2.  The singularity at $z_0$ is a [[Pole]] if, and only if, $\lim_{z \to z_0} |f(z)| = \infty$. ^e6e00d

^rules

## Proof

### First Statement, Removable Singularities

![[#^s1]]

> #### Removable Singularity
> ![[Removable Singularity]]

#### Removable ==> $a_{k < 0} = 0$

To prove the first statement, assume first that $z_0$ is a [[Removable Singularity]] of $f$. Then $f$ has a power series expansion in $B_r(z_0)$, as all $k < 0$ terms in the [[10.1 Laurent Series]] are zero. 

Thus it is bounded in $B_s(z_0)$ for any $s \in (0, r)$. Moreover, the power series gives rise to a [[5.4 Holomorphic Function|Holomorphic Function]] $g : B_r(z_0) \to \C$ that extends $f$.

#### $a_{k < 0} = 0$ ==> Removable

Conversely, suppose that $f$ is bounded in $B_s(z_0)$ for some $s \in (0, r)$. Let $\rho \in (0, s)$. By [[10.2 Laurent's Theorem]], we have a Laurent series expansion

$$
f(z) = \sum_{k = -\infty}^\infty a_k (z - z_0)^k
$$

for $z \in B_r(z_0) \setminus \set{z_0}$, where

$$
a_k = \frac{1}{2\pi i} \int_{\partial B_\rho(z_0)} \frac{f(w)}{(w - z_0)^{k + 1}} \rd w
$$

for all $k \in \Z$. We conclude that

$$
|a_k| \le \frac{1}{\rho^k} \max_{z \in B_s(z_0)} |f(z)|
$$

by [[6.7 Maximum Attained Integral Inequality]]. Letting $\rho \to 0$, we find that $a_k = 0$ for all $k < 0$. Hence we have a removable singularity.

### Second Statement, Poles of order $k_0$

Next we consider the [[#^e6e00d|second statement]] of the theorem.

> ![[10.3 Isolated Singularities#^8f9ba4]]

#### Pole ==> $|f(z \to z_0)| \to \infty$

Suppose first that $z_0$ is a [[Pole]] of $f$. Then there exists $k_0 \in \N$ such that

$$
f(z) = \sum_{k = -k_0}^\infty a_k (z - z_0)^k
$$

for all $z \in B_r(z_0) \setminus \{z_0\}$ and $a_{-k_0} \neq 0$. Define

$$
g(z) = (z - z_0)^{k_0} f(z) = \sum_{k = 0}^\infty a_{k - k_0} (z - z_0)^k.
$$

Then $g$ is continuous at $z_0$, so $\lim_{z \to z_0} g(z) = a_{-k_0}$. Therefore,

$$
\begin{equation*} \lim_{z \to z_0} |f(z)| = \lim_{z \to z_0} \frac{|g(z)|}{|z - z_0|^{k_0}} = \infty. \end{equation*}
$$

#### $|f(z \to z_0)| \to \infty$ ==> Pole

Conversely, suppose that $\lim_{z \to z_0} |f(z)| = \infty$. Then there exists $s > 0$ such that $|f(z)| \ge 1$ for all $z \in B_s(z_0) \setminus \{z_0\}$. 

Therefore, the function 

$$g(z) = \frac{1}{f(z)}$$

is well-defined in $B_s(z_0) \setminus \{z_0\}$. Furthermore, it is [[5.4 Holomorphic Function|Holomorphic]] by the [[5.2 Algebra of Complex Derivatives|Algebra of Complex Derivatives]]. 

Since $\lim_{z \to z_0} |g(z)| = \lim_{z \to z_0} \frac{1}{|f(z)|} = 0$, the singularity of $g$ at $z_0$ is removable by the [[#First Statement Removable Singularities|first statement]]. Hence there exists a power series expansion

$$
g(z) = \sum_{k = 0}^\infty b_k (z - z_0)^k
$$

for $z \in B_s(z_0) \setminus \{z_0\}$. Since $g(0) = \lim_{z \to z_0} g(z) = 0$, we conclude that $b_0 = 0$.

By construction, the function $g$ cannot vanish identically. Hence there exists at least some $k \in \N$ such that $b_k \neq 0$. Let $k_0$ be the smallest index with this property and define

$$
h(z) = \frac{g(z)}{(z - z_0)^{k_0}} = \sum_{k = 0}^\infty b_{k + k_0} (z - z_0)^k.
$$

Then $h$ is [[9.3 Analytic Function|Analytic]], and hence [[5.4 Holomorphic Function|Holomorphic]], in $B_s(z_0)$. 

Moreover, $h(0) = b_{k_0} \neq 0$. Therefore, there exists $s' > 0$ such that $h(z) \neq 0$ in $B_{s'}(z_0)$. It follows that $\frac1{h(z)}$ is also analytic in $B_{s'}(z_0)$. In particular, there exists a power series expansion

$$
\frac{1}{h(z)} = \sum_{k = 0}^\infty c_k (z - z_0)^k,
$$

with $c_0 \neq 0$, for $z \in B_{s'}(z_0)$. Thus

$$
f(z) = \frac{1}{(z - z_0)^{k_0} h(z)} = \sum_{k = -k_0}^\infty c_{k + k_0} (z - z_0)^k.
$$

That is, $z_0$ is a [[Pole]] of order $k_0$ of $f$.